JellyFish logical atomicity proof

jelly_fish/code.v
@@ -1,4 +1,6 @@
-From iris.heap_lang Require Export notation spin_lock.
+From iris.heap_lang Require Import notation.
+
+From SkipList.atomic Require Import proofmode lock.
 
 
 Section node_rep.
@@ -23,7 +25,7 @@ Section node_rep.
   Lemma rep_to_node_inj rep rep':
     rep_to_node rep = rep_to_node rep' → rep = rep'.
   Proof.
-    destruct rep as (((?&?)&?)&?); destruct rep' as (((?&?)&?)&?). 
+    destruct rep as (((?&?)&?)&?); destruct rep' as (((?&?)&?)&?).
     rewrite /rep_to_node/node_key/node_val/node_next/node_lock/=; congruence.
   Qed.
 End node_rep.
@@ -43,7 +45,7 @@ Section val_rep.
   Definition valVT : val := λ: "l", Fst "l".
   Definition valP : val := λ: "l", Snd "l".
 
-  Definition rep_to_val (v: val_rep) : val := 
+  Definition rep_to_val (v: val_rep) : val :=
     (#(val_v v), #(val_t v), #(val_p v)).
   Lemma fold_rep_to_val (v: val_rep) :
     ((#(val_v v), #(val_t v), #(val_p v)))%V =
@@ -69,33 +71,26 @@ End SKIP_LIST_PARAMS.
 
 Module SkipList (Params: SKIP_LIST_PARAMS).
   Import Params.
-  
+
   Definition tail : node_rep := (INT_MAX, dummy_null, dummy_null, dummy_null).
 
-  Definition initLocks : val := 
-    rec: "init" "locks" "lvl" :=
-      if: "lvl" = #(MAX_HEIGHT + 1) then #()
-      else "locks" +ₗ "lvl" <- newlock #();;
-           "init" "locks" ("lvl" + #1).
-
-  Definition new : val := 
-    λ: "_", 
+  Definition new : val :=
+    λ: "_",
       let: "nexts" := AllocN #(MAX_HEIGHT + 1) (ref (rep_to_node tail)) in
-      let: "locks" := AllocN #(MAX_HEIGHT + 1) #() in
-        initLocks "locks" #0;;
+      let: "locks" := AllocN #(MAX_HEIGHT + 1) #false in
         ref (#INT_MIN, #dummy_null, "nexts", "locks").
 
-  Definition find : val := 
+  Definition find : val :=
     rec: "find" "pred" "k" "lvl" :=
       let: "succ" := ! !(nodeNext "pred" +ₗ "lvl") in
         if: "k" ≤ nodeKey "succ" then ("pred", "succ")
         else "find" "succ" "k" "lvl".
-  
-  Definition findLock : val := 
+
+  Definition findLock : val :=
     rec: "find" "pred" "k" "lvl" :=
       let: "pair" := find "pred" "k" "lvl" in
       let: "pred" := Fst "pair" in
-      let: "lock" := !(nodeLock "pred" +ₗ "lvl") in
+      let: "lock" := nodeLock "pred" +ₗ "lvl" in
         acquire "lock";;
         let: "succ" := ! !(nodeNext "pred" +ₗ "lvl") in
           if: "k" ≤ nodeKey "succ" then ("pred", "succ")
@@ -107,7 +102,7 @@ Module SkipList (Params: SKIP_LIST_PARAMS).
       let: "pair" := find "pred" "k" "lvl" in
       let: "pred" := Fst "pair" in
       let: "succ" := Snd "pair" in
-        if: "k" = nodeKey "succ" 
+        if: "k" = nodeKey "succ"
         then let: "val" := !(nodeVal "succ") in SOME (valVT "val")
         else if: "lvl" = #0 then NONEV
              else "find" "pred" "k" ("lvl" - #1).
@@ -115,60 +110,50 @@ Module SkipList (Params: SKIP_LIST_PARAMS).
   Definition get : val :=
     λ: "p" "k", findAll !"p" "k" #MAX_HEIGHT.
 
-  Definition link : val := 
-    λ: "pred" "lvl" "n",
-      let: "new" := !"n" in
-        nodeNext "new" +ₗ "lvl" <- !(nodeNext "pred" +ₗ "lvl") ;;
-        nodeLock "new" +ₗ "lvl" <- newlock #();;
-        nodeNext "pred" +ₗ "lvl" <- "n".
-
-  Definition insert : val := 
+  Definition insert : val :=
     λ: "pred" "lvl" "n",
       let: "k" := nodeKey !"n" in
       let: "pair" := findLock "pred" "k" "lvl" in
       let: "pred" := Fst "pair" in
-      let: "lock" := !(nodeLock "pred" +ₗ "lvl") in
-        link "pred" "lvl" "n";;
+      let: "lock" := nodeLock "pred" +ₗ "lvl" in
+        nodeNext !"n" +ₗ "lvl" <- !(nodeNext "pred" +ₗ "lvl");;
+        nodeNext "pred" +ₗ "lvl" <- "n";;
         release "lock".
 
-  Definition createAndLink : val := 
-    λ: "pred" "k" "v" "t" "h",
-      let: "nexts" := AllocN ("h" + #1) #() in
-      let: "locks" := AllocN ("h" + #1) #() in
-      let: "val" := ref ("v", "t", #dummy_null) in
-      let: "n" := ref ("k", "val", "nexts", "locks") in
-        link "pred" #0 "n";;
-        "n".
-
-  Definition update : val := 
-    λ: "node" "v" "t",
-      let: "val" := !(nodeVal "node") in
-        if: "t" < valT "val" then #()
-        else nodeVal "node" <- ("v", "t", ref "val").
-
-  Definition tryInsert : val := 
+  Definition tryInsert : val :=
     λ: "pred" "k" "v" "t" "h",
       let: "pair" := findLock "pred" "k" #0 in
       let: "pred" := Fst "pair" in
       let: "succ" := Snd "pair" in
-      let: "lock" := !(nodeLock "pred") in
+      let: "lock" := nodeLock "pred" in
         if: "k" = nodeKey "succ"
-        then update "succ" "v" "t";;
-             release "lock";;
-             NONEV
-        else let: "n" := createAndLink "pred" "k" "v" "t" "h" in
+        (* Update existing node *)
+        then let: "val" := !(nodeVal "succ") in
+               if: "t" < valT "val"
+               then release "lock";;
+                    NONEV
+               else nodeVal "succ" <- ("v", "t", ref "val");;
+                    release "lock";;
+                    NONEV
+        (* Allocate and insert new node *)
+        else let: "nexts" := AllocN ("h" + #1) #() in
+             let: "locks" := AllocN ("h" + #1) #false in
+             let: "val" := ref ("v", "t", #dummy_null) in
+             let: "n" := ref ("k", "val", "nexts", "locks") in
+               nodeNext !"n" <- !(nodeNext "pred");;
+               nodeNext "pred" <- "n";;
                release "lock";;
                SOME "n".
 
-  Definition findLevel : val := 
-    rec: "find" "pred" "k" "lvl" "h" := 
+  Definition findLevel : val :=
+    rec: "find" "pred" "k" "lvl" "h" :=
       let: "pair" := find "pred" "k" "lvl" in
       let: "pred" := Fst "pair" in
-        if: "lvl" = "h" then "pair"
+        if: "lvl" = "h" then "pred"
         else "find" "pred" "k" ("lvl" - #1) "h".
 
-  Definition insertAll : val := 
-    rec: "insert" "curr" "k" "v" "t" "h" "lvl" := 
+  Definition insertAll : val :=
+    rec: "insert" "curr" "k" "v" "t" "h" "lvl" :=
       if: "lvl" = #0 then tryInsert "curr" "k" "v" "t" "h"
       else let: "pair" := find "curr" "k" ("lvl" - #1) in
            let: "pred" := Fst "pair" in
@@ -179,19 +164,19 @@ Module SkipList (Params: SKIP_LIST_PARAMS).
                            SOME "n"
              end.
 
-  Definition putH : val := 
+  Definition putH : val :=
     λ: "p" "k" "v" "t" "h",
-      let: "pair" := findLevel !"p" "k" #MAX_HEIGHT "h" in
-      let: "pred" := Fst "pair" in
+      let: "pred" := findLevel !"p" "k" #MAX_HEIGHT "h" in
         insertAll "pred" "k" "v" "t" "h" "h".
 
-  (* HeapLang does not support randomness... *)
+  (* Base HeapLang does not support randomness... *)
   Definition randomLevel : val :=
     λ: "_", #0.
 
   Definition put : val :=
     λ: "p" "k" "v" "t",
       let: "h" := randomLevel #() in
-      let: "_" := putH "p" "k" "v" "t" "h" in #().
+      let: "_" := putH "p" "k" "v" "t" "h" in
+        #().
 
 End SkipList.
