jelly_fish/inv.v
@@ -1,32 +1,30 @@
-From iris.algebra Require Import gmap gset excl_auth dfrac_agree.
-From iris.base_logic.lib Require Import invariants.
-From iris.heap_lang Require Import proofmode.
+From iris.algebra Require Import auth gset.
+From iris.base_logic.lib Require Import ghost_map.
+From iris.heap_lang Require Import notation.
+Import derived_laws_later.bi.
 
-From SkipList.lib Require Import zrange gmap_extra.
+From SkipList.lib Require Import zrange.
+From SkipList.atomic Require Import proofmode lock.
 From SkipList.jelly_fish Require Import code.
 
 
+Definition tval : Type := Z * Z.
+
 Class skipG Σ := SkipG { 
-  skip_authG :> inG Σ (authR (gsetR node_rep));
+  skip_authG :> inG Σ (authR (gset node_rep));
   skip_disjG :> inG Σ (gset_disjR Z);
   skip_toksG :> inG Σ (authR (gset_disjR Z));
-  skip_exclG :> inG Σ (excl_authR (gset Z));
-  skip_valsG :> inG Σ (authR (gmap_disjR Z (Z * Z)));
-  skip_lockG :> lockG Σ
+  skip_gmapG :> ghost_mapG Σ Z (tval * list tval)
 }.
 
-Record inv_gname := mk_inv_gname {
+Record lazy_gname := mk_lazy_gname {
   auth_gname: gname;
   disj_gname: gname;
   toks_gname: gname
 }.
-Global Instance inv_gname_inhabited : Inhabited inv_gname := 
-  populate (mk_inv_gname inhabitant inhabitant inhabitant).
-
-Record map_gname := mk_map_gname {
-  excl_gname: gname;
-  vals_gname: gname
-}.
+(* Necessary to support total lookup (m !!! k) *)
+Global Instance lazy_gname_inhabited : Inhabited lazy_gname := 
+  populate (mk_lazy_gname inhabitant inhabitant inhabitant).
 
 Module SkipListInv (Params: SKIP_LIST_PARAMS).
   Import Params.
@@ -34,167 +32,293 @@ Module SkipListInv (Params: SKIP_LIST_PARAMS).
   Export SkipList.
 
   Section invariant.
-    Context `{!heapGS Σ, !skipG Σ} (N: namespace).
+    Context `{!heapGS Σ, !skipG Σ}.
     Local Open Scope Z.
 
-    Definition locked_val (lvl: Z) (n: loc) : iProp Σ := 
-      if decide (lvl = 0) then 
-        (∃ (node: node_rep), n ↦□ rep_to_node node ∗
-        (⌜ node = tail ⌝ ∨ ∃ (val: val_rep), (node_val node) ↦{#1 / 2} rep_to_val val))%I
-      else True%I.
-    Definition in_lock (lvl: Z) (a: loc) : iProp Σ := 
-      ∃ (n: loc), (a +ₗ lvl) ↦{#1 / 2} #n ∗ locked_val lvl n.
-    Definition has_lock (lvl: Z) (node: node_rep) : iProp Σ := 
-      ∃ (γl: gname) (l: val), 
-        (node_lock node +ₗ lvl) ↦□ l
-        ∗
-        is_lock γl l (in_lock lvl (node_next node)).
-
-    Definition has_next (lvl: Z) (Γi: inv_gname) (pred: node_rep) : iProp Σ :=
+    (* Successor chain *)
+    Definition has_next (lvl: Z) (Γ: lazy_gname) (pred: node_rep) : iProp Σ :=
       ∃ (s: loc) (succ: node_rep), 
         (node_next pred +ₗ lvl) ↦{#1 / 2} #s
         ∗
         s ↦□ rep_to_node succ
         ∗
-        (⌜ succ = tail ⌝ ∨ own Γi.(auth_gname) (◯ {[succ]}))
+        (⌜ succ = tail ⌝ ∨ own Γ.(auth_gname) (◯ {[succ]}))
         ∗
-        own Γi.(disj_gname) (ZRange (node_key pred) (node_key succ)).
+        own Γ.(disj_gname) (ZRange (node_key pred) (node_key succ)).
 
-    Definition has_val (Γm: map_gname) (node: node_rep) : iProp Σ :=
-      ∃ (val: val_rep),
-        (node_val node) ↦{#1 / 2} rep_to_val val
-        ∗
-        own Γm.(vals_gname) (◯ DMap {[ node_key node := (val_vt val)]}).
-    Definition own_map (S: gset node_rep) (Γm: map_gname) : iProp Σ :=
-      own Γm.(excl_gname) (●E (set_map node_key S))
+    (* Lock resources *)
+    Definition locked_val (lvl: Z) (s: loc) : iProp Σ := 
+      if decide (lvl = 0) then 
+        (∃ (succ: node_rep), s ↦□ rep_to_node succ ∗
+        (⌜ succ = tail ⌝ ∨ ∃ (val: val_rep), node_val succ ↦{#1 / 2} rep_to_val val))%I
+      else True%I.
+    Definition in_lock (lvl: Z) (pred: node_rep) : iProp Σ := 
+      ∃ (s: loc), (node_next pred +ₗ lvl) ↦{#1 / 2} #s ∗ locked_val lvl s.
+    Definition has_lock (lvl: Z) (pred: node_rep) : iProp Σ := 
+      is_lock #(node_lock pred +ₗ lvl) (in_lock lvl pred).
+
+    (* Sublist resources *)
+    Definition has_sub (γ: lazy_gname) (node: node_rep) : iProp Σ :=
+      own γ.(auth_gname) (◯ {[ node ]})
       ∗
-      [∗ set] n ∈ S, has_val Γm n.
+      own γ.(toks_gname) (◯ GSet {[ node_key node ]}).
 
-    Definition has_frag (γi: inv_gname) (node: node_rep) : iProp Σ :=
-      own γi.(auth_gname) (◯ {[ node ]})
+    (* Lazy list resources for a given level *)
+    Definition lazy_list (head: node_rep) (S: gset node_rep)
+      (Γ: lazy_gname) (γ: option lazy_gname) (lvl: Z) : iProp Σ :=
+      own Γ.(auth_gname) (● S)
       ∗
-      own γi.(toks_gname) (◯ GSet {[ node_key node ]}).
+      own Γ.(disj_gname) (GSet (set_map node_key S))
+      ∗
+      own Γ.(toks_gname) (● GSet (set_map node_key S))
+      ∗
+      ([∗ set] n ∈ {[head]} ∪ S, has_next lvl Γ n)
+      ∗
+      ([∗ set] n ∈ {[head]} ∪ S, has_lock lvl n)
+      ∗
+      match γ with None => True | Some γ => [∗ set] n ∈ S, has_sub γ n end.
 
-    Definition lazy_list_inv (head: node_rep) (Γm: map_gname) (Γ: gmap Z inv_gname) (lvl: Z) : iProp Σ :=
-      ∃ (S: gset node_rep),
-        own (Γ !!! lvl).(auth_gname) (● S)
+    (* Vertical list resources *)
+    Fixpoint vertical_list (vl: list tval) (p: loc) : iProp Σ := 
+      match vl with
+      | nil => ⌜ p = dummy_null ⌝
+      | vt :: vl => ∃ (n: loc), p ↦□ rep_to_val (vt, n)%core ∗ vertical_list vl n
+      end.
+    Definition has_val (γ: gname) (node: node_rep) : iProp Σ :=
+      ∃ (val: val_rep) (vl: list tval),
+        node_val node ↦{#1 / 2} rep_to_val val
         ∗
-        own (Γ !!! lvl).(disj_gname) (GSet (set_map node_key S))
+        node_key node ↪[γ] (val_vt val, vl)
         ∗
-        own (Γ !!! lvl).(toks_gname) (● GSet (set_map node_key S))
-        ∗
-        ([∗ set] n ∈ {[head]} ∪ S, has_lock lvl n)
-        ∗
-        ([∗ set] n ∈ {[head]} ∪ S, has_next lvl (Γ !!! lvl) n)
-        ∗
-        if decide (lvl = 0) then own_map S Γm
-        else [∗ set] n ∈ S, has_frag (Γ !!! (lvl - 1)) n.
-    Definition skip_list_inv (head: node_rep) (Γm: map_gname) (Γ: gmap Z inv_gname) : iProp Σ :=
-      [∗ set] i ∈ zrange (-1) (MAX_HEIGHT + 1), lazy_list_inv head Γm Γ i.
+        vertical_list vl (val_p val).
 
-    Definition skipN := N .@ "skip".
-    Definition map_inv (p: loc) (Γm: map_gname) : iProp Σ :=
-      ∃ (head: node_rep) (Γ: gmap Z inv_gname),
+    (* JellyFish map resources *)
+    Definition jf_map (head: node_rep) (S: gset node_rep) 
+      (m: gmap Z (tval * list tval)) (Γ: lazy_gname) : iProp Σ :=
+      lazy_list head S Γ None 0
+      ∗
+      ∃ (γ: gname),
+        ⌜ dom m = set_map node_key S ⌝
+        ∗
+        ghost_map_auth γ 1 m
+        ∗
+        [∗ set] n ∈ S, has_val γ n.
+
+    (* Skip list resources *)
+    Definition is_lazy_list (head: node_rep) (Γ: lazy_gname)
+      (γ: lazy_gname) (lvl: Z) : iProp Σ :=
+      ∃ (S: gset node_rep), lazy_list head S Γ (Some γ) lvl.
+    Definition skip_list (head: node_rep) (S: gset node_rep)
+      (m: gmap Z (tval * list tval)) (mΓ: gmap Z lazy_gname) : iProp Σ :=
+      jf_map head S m (mΓ !!! 0)
+      ∗
+      [∗ set] i ∈ zrange 0 (MAX_HEIGHT + 1), 
+        is_lazy_list head (mΓ !!! i) (mΓ !!! (i - 1)) i.
+
+    (* Representation predicate for maps with version control *)
+    Definition vc_map (p: loc) (m: gmap Z (tval * list tval))
+      (mΓ: gmap Z lazy_gname) : iProp Σ :=
+      ∃ (head: node_rep) (S: gset node_rep),
         p ↦□ rep_to_node head
         ∗
         ⌜ node_key head = INT_MIN ⌝
         ∗
-        inv skipN (skip_list_inv head Γm Γ).
+        skip_list head S m mΓ.
 
-    Definition map (m: gmap Z (Z * Z)) (Γm: map_gname) : iProp Σ := 
-      own Γm.(excl_gname) (◯E (dom m))
-      ∗
-      own Γm.(vals_gname) (● DMap m).
-
+    (* Needed for [vc_map] to be timeless *)
+    Global Instance vl_timeless vl p : Timeless (vertical_list vl p).
+    Proof. revert p; induction vl; apply _. Qed.
+    Global Instance locked_val_timeless i l : Timeless (locked_val i l).
+    Proof. unfold locked_val; case_decide; apply _. Qed.
   End invariant.
 
   Section proofs.
-    Context `{!heapGS Σ, !skipG Σ} (N: namespace).
+    Context `{!heapGS Σ, !skipG Σ}.
     Local Open Scope Z.
 
-    Lemma singleton_frag_in (S: gset node_rep) (n s: node_rep) (γ: gname) :
-      own γ (● S) -∗ ⌜ n = s ⌝ ∨ own γ (◯ {[n]}) → ⌜ n ∈ {[s]} ∪ S ⌝.
+    Lemma singleton_frag_in (h n s: node_rep) (S: gset node_rep) (Γ: lazy_gname) 
+      (γ: option lazy_gname) (lvl: Z) :
+      ⌜ n = s ⌝ ∨ own Γ.(auth_gname) (◯ {[n]}) -∗ 
+      lazy_list h S Γ γ lvl -∗ 
+      ⌜ n ∈ {[s]} ∪ S ⌝.
     Proof.
-      iIntros "Hauth Hnode".
+      iIntros "Hnode Hlazy".
+      iDestruct "Hlazy" as "(Hauth & Hdisj & Htoks & Hnexts & Hlocks & Hsubs)".
       iDestruct "Hnode" as "[->|Hnode]"; first (iPureIntro; set_solver).
       iDestruct (own_valid_2 with "Hauth Hnode") 
         as %[?%gset_included]%auth_both_valid_discrete.
       iPureIntro; set_solver.
     Qed.
 
-    Lemma has_lvl_inv (lvl: Z) (head: node_rep) 
-      (Γm: map_gname) (Γ: gmap Z inv_gname) :
-      0 ≤ lvl ≤ MAX_HEIGHT →
-      skip_list_inv head Γm Γ ⊢
-        lazy_list_inv head Γm Γ lvl
-        ∗
-        (lazy_list_inv head Γm Γ lvl -∗ skip_list_inv head Γm Γ).
-    Proof.
-      intros Hlvl; unfold skip_list_inv.
-      rewrite (big_sepS_delete _ _ lvl); last (rewrite zrange_spec; lia).
-      iIntros "(Hlvl & Hskip)"; iFrame; by iIntros.
-    Qed.
-
-    Lemma frag_has_val (lvl: Z) (head node: node_rep) 
-      (Γm: map_gname) (Γ: gmap Z inv_gname) :
-      0 ≤ lvl ≤ MAX_HEIGHT →
-      skip_list_inv head Γm Γ -∗
-      own (Γ !!! lvl).(auth_gname) (◯ {[node]}) -∗
-          has_val Γm node
+    Lemma node_has_next (head pred: node_rep) (S: gset node_rep) (Γ: lazy_gname)
+      (γ: option lazy_gname) (lvl: Z) :
+      ⌜ pred = head ⌝ ∨ own Γ.(auth_gname) (◯ {[pred]}) -∗
+      lazy_list head S Γ γ lvl -∗
+        ∃ (s: loc) (succ: node_rep), 
+          (node_next pred +ₗ lvl) ↦{#1 / 2} #s
           ∗
-          (has_val Γm node -∗ skip_list_inv head Γm Γ).
+          s ↦□ rep_to_node succ
+          ∗
+          (⌜ succ = tail ⌝ ∨ own Γ.(auth_gname) (◯ {[succ]}))
+          ∗
+          ⌜ set_map node_key S ## zrange (node_key pred) (node_key succ) ⌝
+          ∗
+          ((node_next pred +ₗ lvl) ↦{#1 / 2} #s -∗ lazy_list head S Γ γ lvl).
     Proof.
-      iIntros (Hlvl) "Hskip Hnode".
-      assert (lvl = Z.of_nat (Z.to_nat lvl)) as Heq by lia.
-      iRevert (Hlvl) "Hnode"; rewrite Heq; clear Heq.
-      iInduction (Z.to_nat lvl) as [|lvl'] "Himp"; iIntros "%Hlvl Hnode".
-      + iDestruct (has_lvl_inv 0 with "Hskip") as "(Hlvl & Hskip)"; first (pose HMAX_HEIGHT; lia).
-        iDestruct "Hlvl" as (S) "(Hauth & ? & ? & ? & ? & Hmap)".
-        iDestruct (own_valid_2 with "Hauth Hnode") as %[?%gset_included]%auth_both_valid_discrete.
-        iDestruct "Hmap" as "(Hexcl● & Hvals◯)".
-        rewrite (big_sepS_delete (has_val _) _ node); last set_solver.
-        iDestruct "Hvals◯" as "(Hval & Hvals◯)"; iFrame.
-        iIntros "Hval"; iCombine "Hval Hvals◯" as "Hvals◯". 
-        rewrite -big_sepS_delete; last set_solver.
-        iApply "Hskip"; iExists S; iFrame.
-      + iDestruct (has_lvl_inv with "Hskip") as "(Hlvl & Hskip)"; first done.
-        iDestruct "Hlvl" as (S) "(Hauth & ? & ? & ? & ? & Hfrags)".
-        case_decide; first lia.
-        iDestruct (own_valid_2 with "Hauth Hnode") as %[?%gset_included]%auth_both_valid_discrete.
-        rewrite (big_sepS_delete (has_frag _) _ node); last set_solver.
-        iDestruct "Hfrags" as "((#Hnode' & ?) & Hfrags)".
-        iAssert (has_frag _ _) with "[$]" as "Hfrag".
-        iCombine "Hfrag Hfrags" as "Hfrags".
-        rewrite -(big_sepS_delete (has_frag _)); last set_solver.
-        replace (Z.of_nat lvl') with (Datatypes.S lvl' - 1) by lia.
-        iApply ("Himp" with "[-] [%] [$]"); last lia.
-        iApply "Hskip". iExists S; case_decide; first lia; iFrame.
+      iIntros "#Hpred Hlazy".
+      iDestruct (singleton_frag_in with "Hpred Hlazy") as %Hpred.
+      iDestruct "Hlazy" as "(Hauth & Hdisj & Htoks & Hnexts & Hlocks & Hsubs)".
+      rewrite (big_sepS_delete (has_next lvl Γ) _ pred) //.
+      iDestruct "Hnexts" as "(Hnext & Hnexts)".
+      iDestruct "Hnext" as (s succ) "(Hnext & #Hs & #Hsucc & Hkeys)".
+      iDestruct (own_valid_2 with "Hdisj Hkeys") as %[Hdisj _]%ZRange_disj.
+
+      iExists s, succ; iFrame "# ∗"; iSplit; first done. iIntros "Hnext". 
+      iAssert (has_next lvl Γ pred) with "[Hnext Hkeys]" as "Hnext".
+      { iExists s, succ; iFrame "# ∗". }
+      iCombine "Hnext Hnexts" as "Hnexts"; rewrite -big_sepS_delete //.
     Qed.
 
-    Lemma has_lower_frag (lvl: Z) (head node: node_rep) 
-      (Γm: map_gname) (Γ: gmap Z inv_gname) :
-      0 < lvl ≤ MAX_HEIGHT →
-      inv (skipN N) (skip_list_inv head Γm Γ) -∗
-      ⌜ node = head ⌝ ∨ own (auth_gname (Γ !!! lvl)) (◯ {[node]}) ={⊤}=∗
-      ⌜ node = head ⌝ ∨ own (auth_gname (Γ !!! (lvl - 1))) (◯ {[node]}).
+    Lemma node_has_lock (head node: node_rep) (S: gset node_rep) (Γ: lazy_gname)
+      (γ: option lazy_gname) (lvl: Z) :
+      ⌜ node = head ⌝ ∨ own Γ.(auth_gname) (◯ {[node]}) -∗
+      lazy_list head S Γ γ lvl -∗
+        has_lock lvl node ∗ (has_lock lvl node -∗ lazy_list head S Γ γ lvl).
     Proof.
-      iIntros (Hlvl) "#Hinv Hnode".
-      iDestruct "Hnode" as "[->|Hnode]"; first by (iModIntro; iLeft).
-      iInv "Hinv" as "Hskip".
-      iDestruct (has_lvl_inv lvl with "Hskip") as "(Hlvl & Hskip)"; first lia.
-      iDestruct "Hlvl" as (S) "(>Hauth & ? & ? & ? & ? & Hfrags)".
-      case_decide; first lia; iMod "Hfrags".
+      iIntros "#Hnode Hlazy".
+      iDestruct (singleton_frag_in with "Hnode Hlazy") as %Hnode.
+      iDestruct "Hlazy" as "(Hauth & Hdisj & Htoks & Hnexts & Hlocks & Hsubs)".
+      rewrite (big_sepS_delete (has_lock lvl) _ node) //.
+      iDestruct "Hlocks" as "(Hlock & Hlocks)".
+      iFrame; iIntros "Hlock".
+      iCombine "Hlock Hlocks" as "Hlocks"; rewrite -big_sepS_delete //.
+    Qed.
 
+    Definition opt_sub (mΓ: gmap Z lazy_gname) (lvl: Z) : option lazy_gname :=
+      if decide (lvl = 0) then None
+      else Some (mΓ !!! (lvl - 1)).
+    Lemma skip_has_lazy (lvl: Z) (head: node_rep) 
+      (S: gset node_rep) (m: gmap Z (tval * list tval))
+      (mΓ: gmap Z lazy_gname) :
+      0 ≤ lvl ≤ MAX_HEIGHT →
+      skip_list head S m mΓ ⊢
+        ∃ (S': gset node_rep),
+          lazy_list head S' (mΓ !!! lvl) (opt_sub mΓ lvl) lvl
+          ∗ (
+            lazy_list head S' (mΓ !!! lvl) (opt_sub mΓ lvl) lvl 
+            -∗ 
+            skip_list head S m mΓ
+          )
+          ∗
+          ⌜ lvl = 0 → dom m = set_map node_key S' ⌝.
+    Proof.
+      iIntros "%Hlvl [[Hbot Hmap] Hskip]".
+      destruct (Z.to_nat lvl) as [|lvl'] eqn:Heq.
+      + replace lvl with 0 by lia. iExists S.
+        iDestruct "Hmap" as (γ) "(%Hdom & Hauth & Hvals)".
+        iFrame "Hbot". iSplit; last by iPureIntro.
+        iIntros. iFrame. iExists γ. by iFrame.
+      + rewrite (big_sepS_delete _ _ lvl); last (rewrite zrange_spec; lia).
+        iDestruct "Hskip" as "[[%S' Hlazy] Hskip]".
+        iExists S'. unfold opt_sub; case_decide; first lia.
+        iFrame. iSplit; last by iPureIntro. iIntros "Hlazy".
+        iApply (big_sepS_delete _ _ lvl); first (rewrite zrange_spec; lia).
+        iFrame. by iExists S'.
+    Qed.
+
+    Lemma node_in_lower (lvl: Z) (h n: node_rep)
+      (S: gset node_rep) (m: gmap Z (tval * list tval))
+      (mΓ: gmap Z lazy_gname) :
+      1 ≤ lvl ≤ MAX_HEIGHT → 
+      skip_list h S m mΓ -∗
+      own (mΓ !!! lvl).(auth_gname) (◯ {[n]}) -∗
+      own (mΓ !!! (lvl - 1)).(auth_gname) (◯ {[n]}).
+    Proof.
+      iIntros (Hlvl) "[[Hbot Hmap] Hskip] #Hnode".
+      rewrite (big_sepS_delete _ _ lvl); last (rewrite zrange_spec; lia).
+      iDestruct "Hskip" as "[[%S' Hlazy] Hskip]".
+      iDestruct "Hlazy" as "(Hauth & Hdisj & Htoks & Hnexts & Hlocks & Hsubs)".
       iDestruct (own_valid_2 with "Hauth Hnode") 
         as %[?%gset_included]%auth_both_valid_discrete.
-      rewrite (big_sepS_delete (has_frag _) _ node); last set_solver.
-      iDestruct "Hfrags" as "((#Hnode' & ?) & Hfrags)".
-      iAssert (has_frag _ _) with "[$]" as "Hfrag".
-      iCombine "Hfrag Hfrags" as "Hfrags".
-      rewrite -(big_sepS_delete (has_frag _)); last set_solver.
-
-      iModIntro; iSplitR ""; last (iModIntro; iFrame "Hnode'").
-      iNext; iApply "Hskip"; iExists S; case_decide; first lia; iFrame.
+      rewrite (big_sepS_delete (has_sub _) _ n); last set_solver.
+      by iDestruct "Hsubs" as "[[#Hfrag Htok] Hsubs]".
     Qed.
+
+    Lemma sent_or_node_in_lower (lvl: Z) (h n s: node_rep) 
+      (S: gset node_rep) (m: gmap Z (tval * list tval))
+      (mΓ: gmap Z lazy_gname) :
+      1 ≤ lvl ≤ MAX_HEIGHT → 
+      skip_list h S m mΓ -∗
+      ⌜ n = s ⌝ ∨ own (mΓ !!! lvl).(auth_gname) (◯ {[n]}) -∗
+      ⌜ n = s ⌝ ∨ own (mΓ !!! (lvl - 1)).(auth_gname) (◯ {[n]}).
+    Proof.
+      iIntros (Hlvl) "Hskip #Hnode".
+      iDestruct "Hnode" as "[->|Hnode]"; first by iLeft. iRight.
+      by iApply (node_in_lower with "Hskip Hnode").
+    Qed.
+
+    Lemma node_in_bot (lvl: Z) (h n: node_rep) 
+      (S: gset node_rep) (m: gmap Z (tval * list tval))
+      (mΓ: gmap Z lazy_gname) :
+      0 ≤ lvl ≤ MAX_HEIGHT →
+      skip_list h S m mΓ -∗
+      own (mΓ !!! lvl).(auth_gname) (◯ {[n]}) -∗
+      own (mΓ !!! 0).(auth_gname) (◯ {[n]}).
+    Proof.
+      iIntros (Hlvl) "Hskip #Hnode".
+      assert (lvl = Z.of_nat (Z.to_nat lvl)) as Heq by lia.
+      iRevert (Hlvl); rewrite Heq; clear Heq.
+      iInduction (Z.to_nat lvl) as [|lvl'] "Himp"; first by iIntros.
+      iIntros "%Hlvl'".
+      iDestruct (node_in_lower with "Hskip Hnode") as "#Hnode'"; first lia.
+      replace (Datatypes.S lvl' - 1) with (Z.of_nat lvl') by lia.
+      iApply ("Himp" with "Hnode' Hskip"). iPureIntro; lia.
+    Qed.
+
+    Lemma node_has_val (lvl: Z) (h n: node_rep) 
+      (S: gset node_rep) (m: gmap Z (tval * list tval))
+      (mΓ: gmap Z lazy_gname) :
+      0 ≤ lvl ≤ MAX_HEIGHT →
+      skip_list h S m mΓ -∗
+      own (mΓ !!! lvl).(auth_gname) (◯ {[n]}) -∗
+      ∃ (val: val_rep) (vl: list tval),
+        node_val n ↦{#1 / 2} rep_to_val val
+        ∗
+        ⌜ m !! node_key n = Some (val_vt val, vl) ⌝
+        ∗
+        (node_val n ↦{#1 / 2} rep_to_val val -∗ skip_list h S m mΓ).
+    Proof.
+      iIntros "%Hlvl Hskip #Hnode".
+      iDestruct (node_in_bot with "Hskip Hnode") as "#Hnode'"; first done.
+      iDestruct "Hskip" as "[[Hlazy Hmap] Hskip]".
+      iDestruct "Hlazy" as "(Hauth & Hdisj & Htoks & Hnexts & Hlocks & Hsubs)".
+      iDestruct (own_valid_2 with "Hauth Hnode'") 
+        as %[?%gset_included]%auth_both_valid_discrete.
+
+      iDestruct "Hmap" as (γ) "(Hdom & Hgmap & Hvals)".
+      rewrite (big_sepS_delete (has_val _) _ n); last set_solver.
+      iDestruct "Hvals" as "[Hval Hvals]".
+      iDestruct "Hval" as (val vl) "(Hpt & Hvt & Hvl)".
+      iDestruct (ghost_map_lookup with "Hgmap Hvt") as %Hsome.
+
+      iExists val, vl. iFrame "Hpt". iSplit; first done.
+      iIntros "Hpt". iFrame. iExists γ. iFrame "Hgmap".
+      iApply (big_sepS_delete _ _ n); first set_solver.
+      iFrame "Hvals". iExists val, vl. iFrame.
+    Qed.
+
+    Lemma map_has_skip (p: loc) (head: node_rep) (m: gmap Z (tval * list tval)) 
+      (mΓ: gmap Z lazy_gname) :
+      p ↦□ rep_to_node head -∗
+      vc_map p m mΓ -∗
+        ∃ (S : gset node_rep), 
+          (skip_list head S m mΓ)
+          ∗ 
+          (skip_list head S m mΓ -∗ vc_map p m mΓ).
+    Proof.
+      iIntros "Hhead Hmap". iDestruct "Hmap" as (h' S) "(#H & %Hmin & Hskip)".
+      iDestruct (mapsto_agree with "Hhead H") as %<-%rep_to_node_inj; iClear "H".
+      iExists S. iFrame "Hskip". iIntros "Hskip". iExists head, S. by iFrame.
+    Qed. 
   End proofs.
 End SkipListInv.
