jelly_fish/spec/get.v
@@ -1,14 +1,10 @@
-From iris.algebra Require Import gmap gset excl_auth dfrac_agree.
-From iris.base_logic.lib Require Import invariants.
-From iris.program_logic Require Import atomic.
-From iris.heap_lang Require Import proofmode.
+From stdpp Require Import numbers.
+From iris.heap_lang Require Import notation.
 
-From SkipList.lib Require Import zrange gmap_extra.
+From SkipList.atomic Require Import weakestpre proofmode.
 From SkipList.jelly_fish Require Import code inv.
 From SkipList.jelly_fish.spec Require Import find.
 
-
-Local Open Scope Z.
 
 Module GetSpec (Params: SKIP_LIST_PARAMS).
   Import Params.
@@ -16,89 +12,113 @@ Module GetSpec (Params: SKIP_LIST_PARAMS).
   Export Find.
 
   Section Proofs.
-    Context `{!heapGS Σ, !skipG Σ} (N: namespace).
+    Context `{!heapGS Σ, !skipG Σ}.
+    Local Open Scope Z.
 
-    Definition opt_to_val (opt: option (Z * Z)) : val :=
+    Definition opt_to_val (opt: option (tval * list tval)) : val :=
       match opt with
       | None => NONEV
-      | Some vt => SOMEV (#vt.1, #vt.2)
+      | Some (v, t, vl) => SOMEV (#v, #t)
       end.
 
-    Theorem findAll_spec (k lvl: Z) (head curr: node_rep) (Γm: map_gname) (Γ: gmap Z inv_gname) :
+    Theorem findAll_spec (k lvl: Z) (head curr: node_rep) (mΓ: gmap Z lazy_gname) :
       node_key curr < k < INT_MAX →
       0 ≤ lvl ≤ MAX_HEIGHT →
-      (⌜ curr = head ⌝ ∨ own (Γ !!! lvl).(auth_gname) (◯ {[curr]})) -∗
-      inv (skipN N) (skip_list_inv head Γm Γ) -∗
-      <<< ∀∀ (m: gmap Z (Z * Z)), map m Γm >>>
-        findAll (rep_to_node curr) #k #lvl @ ↑(skipN N)
-      <<< map m Γm, RET opt_to_val (m !! k) >>>.
+      (⌜ curr = head ⌝ ∨ own (mΓ !!! lvl).(auth_gname) (◯ {[curr]})) -∗
+      <<< ∀∀ S m, skip_list head S m mΓ >>>
+        findAll (rep_to_node curr) #k #lvl @ ∅
+      <<< skip_list head S m mΓ, RET opt_to_val (m !! k) >>>
+      {{{ True }}}.
     Proof.
-      iIntros "%Hk %Hlvl Hcurr #Hinv %Φ"; iRevert (lvl curr Hk Hlvl) "Hcurr".
+      iIntros "%Hk %Hlvl Hcurr %Φ"; iRevert (lvl curr Hk Hlvl) "Hcurr".
       iLöb as "IH"; iIntros (lvl curr Hk Hlvl) "#Hcurr AU".
+      rewrite difference_empty_L.
       wp_lam. wp_let. wp_let.
 
-      awp_apply (find_spec with "Hcurr Hinv"); first done; first done.
-      iApply (aacc_aupd with "AU"); first done.
-      iIntros (m) "(Hexcl◯ & Hvals)"; iAaccIntro with "Hexcl◯".
-      { do 2 (iIntros "?"; iModIntro; iFrame). }
-      iIntros (pred succ) "(Hexcl◯ & %Hnin & #Hpred & #Hsucc & %Hk' & Hlock)".
-      iDestruct "Hlock" as (γl l) "(#Hlock & #His_lock)".
+      awp_apply (find_spec with "Hcurr"); first done.
+      iApply (aacc_aupd_sub with "[] AU"); try done.
+      {
+        iIntros "!> %S %m Hskip".
+        iDestruct (skip_has_lazy with "Hskip") as (S') "[Hlazy [Hskip _]]"; first done.
+        iExists S'. iFrame.
+      }
+      iIntros (S m) "Hskip".
+      iDestruct (skip_has_lazy with "Hskip") as (S') "[Hlazy [Hskip %Hdom]]"; first done.
+      iAaccIntro with "Hlazy".
+      { iIntros "H"; iDestruct ("Hskip" with "H") as "Hskip". iModIntro; iFrame; by iIntros. }
+      iIntros (pred succ) "[Hlazy %Hkin]".
+      iModIntro. iExists S'. iFrame "Hlazy". iIntros "Hlazy".
 
       destruct (decide (k = node_key succ)) as [->|Hneq].
-      + iModIntro; iLeft; iFrame.
-        iIntros "AU"; iModIntro.
-        wp_pures; wp_lam; wp_pures.
+      + iLeft. iDestruct ("Hskip" with "Hlazy") as "Hskip". iFrame.
+        clear dependent S S' m. iIntros "AU".
+        iModIntro. iIntros "(Hpred & #Hsucc & %Hk')".
+        iModIntro. wp_pures; wp_lam; wp_pures.
         case_bool_decide; last congruence.
         wp_pures; wp_lam; wp_pures.
-
-        wp_bind (Load _). iInv "Hinv" as "Hskip".
-        iDestruct "Hsucc" as "[->|Hsucc]"; first (rewrite /node_key/= in Hk; lia).
-        iDestruct (frag_has_val with "Hskip []") as "(>Hval & Hskip)"; first done.
-        { by iNext. }
-
-        clear dependent m; iMod "AU" as (m) "[(Hexcl◯ & Hvals●) [_ Hclose]]".
-        iDestruct "Hval" as (v) "(Hpt & Hval)".
-        iDestruct (own_valid_2 with "Hvals● Hval") 
-          as %[->%gmap_disj_included%map_singleton_subseteq_l]%auth_both_valid_discrete.
-
-        wp_load.
-        iDestruct ("Hclose" with "[$]") as ">HΦ"; last iModIntro.
-        iModIntro; iSplitL "Hskip Hpt Hval".
-        { iNext; iApply "Hskip"; iExists v; iFrame. }
-        by wp_let; wp_lam; wp_pures.
+        wp_bind (Load _). iMod "AU" as (S m) "[Hskip [_ Hclose]]".
+        iDestruct "Hsucc" as "[->|Hsucc]"; first (rewrite /node_key/tail/= in Hk; lia).
+        iDestruct (node_has_val with "Hskip Hsucc") 
+          as (val vl) "(Hval & %Heq & Hskip)"; first done.
+        wp_load. iDestruct ("Hskip" with "Hval") as "Hskip".
+        iMod ("Hclose" with "Hskip") as "AP".
+        destruct val as [[]]; rewrite Heq.
+        iMod (atomic_post_commit with "AP") as "HΦ".
+        iModIntro. wp_let; wp_lam; wp_pures.
+        by iApply "HΦ".
       + destruct (decide (lvl = 0)) as [->|].
-        - iModIntro; iRight; iFrame.
-          iIntros "HΦ"; iModIntro.
-          wp_pures; wp_lam; wp_pures.
+        - iRight. iDestruct ("Hskip" with "Hlazy") as "Hskip". iFrame.
+          assert (m !! k = None) as ->.
+          { by apply not_elem_of_dom; rewrite Hdom //=; apply Hkin. }
+          clear dependent S S' m. iIntros "AP".
+          iMod (atomic_post_commit with "AP") as "HΦ".
+          iModIntro. iIntros "(Hpred & Hsucc & %Hk')".
+          iModIntro. wp_pures; wp_lam; wp_pures.
           case_bool_decide; first congruence.
-          wp_pures; iModIntro. 
-          replace (m !! k) with (@None (Z * Z)); first done.
-          symmetry; by apply not_elem_of_dom, Hnin.
-        - iModIntro; iLeft; iFrame.
-          iIntros "AU"; iModIntro.
-          wp_pures; wp_lam; wp_pures.
+          wp_pures. by iApply "HΦ".
+        - iLeft. iDestruct ("Hskip" with "Hlazy") as "Hskip". iFrame.
+          clear dependent S S' m. iIntros "AU".
+          iModIntro. iIntros "(Hpred & Hsucc & %Hk')".
+          iMod "AU" as (S m) "[Hskip [Hclose _]]".
+          iDestruct (sent_or_node_in_lower with "Hskip Hpred") as "#Hpred'"; first lia.
+          iMod ("Hclose" with "[$]") as "AU".
+          iModIntro. wp_pures; wp_lam; wp_pures.
           do 2 (case_bool_decide; first congruence; wp_pures).
-          iDestruct (has_lower_frag with "Hinv Hpred") as ">Hpred'"; first lia.          
-          by iApply ("IH" with "[%] [%] Hpred'"); first lia; first lia.
+          iApply ("IH" with "[%] [%] Hpred' AU"); first lia; first lia.
     Qed.
 
-    Theorem get_spec (p: loc) (Γm: map_gname)
+    Theorem get_spec (p: loc) (mΓ: gmap Z lazy_gname)
       (k: Z) (Hrange: INT_MIN < k < INT_MAX) :
-      map_inv N p Γm -∗
-      <<< ∀∀ (m: gmap Z (Z * Z)), map m Γm >>>
-        get #p #k @ ↑(skipN N)
-      <<< map m Γm, RET opt_to_val (m !! k) >>>.
+      ⊢ <<< ∀∀ (m: gmap Z (tval * list tval)), vc_map p m mΓ >>>
+        get #p #k @ ∅
+      <<< vc_map p m mΓ, RET opt_to_val (m !! k) >>>
+      {{{ True }}}.
     Proof.
-      iIntros "#H %Φ AU".
-      iDestruct "H" as (head Γ) "(Hp & %Hmin & #Hinv)".
-      wp_lam. wp_let. wp_load.
+      iIntros (Φ) "AU".
+      wp_lam. wp_let.
 
-      awp_apply (findAll_spec with "[] Hinv"); 
+      wp_bind (Load _). iMod "AU" as (m) "[Hmap [Hclose _]]".
+      iDestruct "Hmap" as (head S) "(#Hhead & %Hmin & Hskip)".
+      wp_load. iDestruct ("Hclose" with "[Hskip]") as ">AU".
+      { iExists head, S; by iFrame "# ∗". }
+      iModIntro; clear dependent m S.
+
+      awp_apply (findAll_spec with "[]"); 
         first lia; first (pose HMAX_HEIGHT; lia); first by iLeft.
-      iApply (aacc_aupd with "AU"); first done.
-      iIntros (m) "Hmap"; iAaccIntro with "Hmap".
-      { do 2 (iIntros "?"; iModIntro; iFrame). }
-      iIntros. iModIntro; iRight; iFrame. by iIntros.
+      iApply (aacc_aupd_sub with "[] AU"); try done.
+      { 
+        iIntros "!> %m Hmap". 
+        iDestruct (map_has_skip with "Hhead Hmap") as (S) "?". 
+        iExists S, m. iFrame. 
+      }
+      iIntros (m) "Hmap". 
+      iDestruct (map_has_skip with "Hhead Hmap") as (S) "[Hskip Hmap]".
+      iAaccIntro with "Hskip".
+      { iIntros "H"; iDestruct ("Hmap" with "H") as "Hmap"; iModIntro; iFrame; by iIntros. }
+      iIntros "H". iModIntro. iExists S, m. iFrame "H".
+      iIntros "Hskip". iDestruct ("Hmap" with "Hskip") as "Hmap".
+      iRight. iFrame "Hmap". iIntros "AP".
+      by iMod (atomic_post_commit with "AP") as "HΦ".
     Qed.
   End Proofs.
 End GetSpec.
