jelly_fish/spec/insert.v
@@ -1,344 +1,409 @@
-From iris.base_logic.lib Require Import invariants.
-From iris.algebra Require Import auth frac_auth gmap gset.
-From iris.heap_lang Require Import proofmode.
+From iris.algebra Require Import auth gset.
+From iris.base_logic.lib Require Import ghost_map.
+From iris.heap_lang Require Import notation.
 
-From SkipList.lib Require Import arg_max.
-From SkipList.jelly_fish Require Import code.
-From SkipList.lib Require Import misc node_rep node_lt.
-From SkipList.jelly_fish.inv Require Import list_equiv lazy_inv skip_inv.
-From SkipList.jelly_fish.spec Require Import link.
+From SkipList.lib Require Import zrange.
+From SkipList.atomic Require Import weakestpre proofmode lock.
+From SkipList.jelly_fish Require Import code inv.
+From SkipList.jelly_fish.spec Require Import find.
 
-
-Local Open Scope Z.
 
 Module InsertSpec (Params: SKIP_LIST_PARAMS).
   Import Params.
-  Module Link := LinkSpec Params.
-  Export Link.
+  Module Find := FindSpec Params.
+  Export Find.
+
+  Definition case_set (S: gset node_rep) (node: node_rep)
+    (m: gmap Z (tval * list tval)) (k: Z) : gset node_rep :=
+    match m !! k with
+    | None => S ∪ {[ node ]}
+    | Some _ => S
+    end.
+
+  Definition case_map (m: gmap Z (tval * list tval)) (k v t: Z) : gmap Z (tval * list tval) :=
+    match m !! k with
+    | None => <[k := (v, t, nil)]> m
+    | Some (vt, vl) => if decide (Z.lt t vt.2) then m
+                       else <[k := (v, t, vt :: vl)]> m
+    end.
 
   Section Proofs.
-    Context `{!heapGS Σ, !skipGS Σ, !lockG Σ}.
+    Context `{!heapGS Σ, !skipG Σ}.
+    Local Open Scope Z.
 
-    Theorem update_spec (v t: Z) (head node: node_rep) 
-      (M: gmap Z (argmax Z)) (q: frac)
-      (bot: bot_gname) (Γ: sub_gname) 
-      (val: val_rep) :
+    Theorem insert_spec (head curr new: node_rep) (n: loc)
+      (Γ γ: lazy_gname) (lvl: Z) :
+      0 < lvl →
+      node_key head < node_key new < INT_MAX →
+      node_key curr < node_key new →
+      (⌜ curr = head ⌝ ∨ own Γ.(auth_gname) (◯ {[ curr ]})) -∗
+      n ↦□ rep_to_node new -∗
+      (node_next new +ₗ lvl) ↦ #() -∗
+      (node_lock new +ₗ lvl) ↦ #false -∗
+      has_sub γ new -∗
+      <<< ∀∀ (S: gset node_rep), lazy_list head S Γ (Some γ) lvl >>>
+        insert (rep_to_node curr) #lvl #n @ ∅
+      <<< lazy_list head (S ∪ {[ new ]}) Γ (Some γ) lvl, RET #() >>>
       {{{
-        inv (levelN 0) (lazy_list_inv 0 head (Some bot) Γ None)
-        ∗
-        own (s_frac bot) (◯F{q} M)
-        ∗
-        own (s_auth Γ) (◯ {[ node ]})
-        ∗
-        (node_val node) ↦{#1 / 2} rep_to_val val
-      }}}
-        update (rep_to_node node) #v #t
-      {{{ val', RET #();
-        own (s_frac bot) (◯F{q} (M ⋅ {[ node_key node := prodZ {[ v ]} t ]}))
-        ∗
-        (node_val node) ↦{#1 / 2} rep_to_val val'
-        ∗
-        if decide (t < val_ts val) then ⌜ val = val' ⌝  
-                                    else ⌜ val_v val' = v ⌝
-                                         ∗
-                                         ⌜ val_ts val' = t ⌝
-                                         ∗
-                                         (val_prev val') ↦□ rep_to_val val
+        has_sub Γ new
       }}}.
     Proof.
-      iIntros (Φ) "(#Hinv & Hown_frag & #Hown_succ & Hval) HΦ".
-      wp_lam. wp_pures. wp_lam. wp_pures.
-      wp_load. wp_let. wp_lam. wp_pures.
+      iIntros "%Hlvl %Hk %Hk' #Hcurr #Hn Hnew Hlock [Hfrag' Htok'] %Φ AU".
+      wp_lam; wp_pures. wp_load. wp_lam; wp_pures.
 
-      case_bool_decide; wp_if.
-      + iInv (levelN 0) as (M' S' L) "(Hinv_sub & >Hown_frac & >%Hequiv)" "Hclose".
-        iDestruct "Hinv_sub" as "(>%Hperm & >%Hsort & >Hown_auth & >Hown_toks & Hlist)".
+      awp_apply (findLock_spec with "Hcurr"); first lia.
+      iApply (aacc_aupd_eq with "AU"); try done.
+      iIntros (S) "Hlazy"; iAaccIntro with "Hlazy".
+      { iIntros; iModIntro; iFrame; by iIntros. }
+      iIntros (pred succ) "[Hlazy %Hnin]".
+      iModIntro. iExists S. iFrame "Hlazy". iIntros "Hlazy".
+      iLeft. iFrame "Hlazy". iIntros "AU". clear dependent S.
+      iModIntro. iIntros "(#Hpred & #Hsucc & %Hk'' & Hlocked)".
+      iDestruct "Hlocked" as (s) "(Hpt & #Hs & _ & Hlocked)".
+      iModIntro. wp_pures; wp_lam; wp_pures; wp_lam; wp_pures.
+      wp_load. wp_load. wp_lam; wp_pures.
+      wp_store. iDestruct "Hnew" as "[Hnew Hnew']".
+      wp_lam; wp_pures.
 
-        iAssert ⌜ In node L ⌝%I with "[Hown_auth]" as %Hin.
-        {
-          iDestruct (own_valid_2 with "Hown_auth Hown_succ") 
-            as %[Hvalid%gset_included]%auth_both_valid_discrete.
-          rewrite -elem_of_list_In Hperm elem_of_elements.
-          iPureIntro; set_solver.
-        }
+      wp_bind (Store _ _). iMod "AU" as (S) "[Hlazy [_ Hclose]]".
+      iDestruct (singleton_frag_in with "Hpred Hlazy") as %Hpred.
+      iDestruct "Hlazy" as "(Hauth & Hdisj & Htoks & Hnexts & Hlocks & Hsubs)".
 
-        rewrite list_equiv_invert_L; last done.
-        iDestruct "Hlist" as (val' γ l s succ) "(_ & Hpt & _ & _ & _ & >Hnode & >%Hval & Himp)".
-        iDestruct (mapsto_agree with "Hval Hnode") as %<-%rep_to_val_inj.
-        destruct Hval as [vs [Hsome Hv]].
-
-        assert (M ⋅ ∅ = M) as <- by rewrite right_id_L //.
-        rewrite -(Qp.div_2 q) frac_auth_frag_op.
-        iDestruct "Hown_frag" as "(Hown_frag & Hown_emp)".
-        iMod (own_update_2 with "Hown_frac Hown_emp") as "[Hown_frac Hown_emp]".
-        { 
-          apply frac_auth_update. 
-          apply (insert_alloc_local_update _ _ 
-            (node_key node) 
-            (prodZ vs (val_ts val)) 
-            (prodZ {[v]} t ⋅ prodZ vs (val_ts val)) 
-            (prodZ {[v]} t)
-          ); auto.
-          apply arg_max_local_update.
-        }
-
-        rewrite arg_max_lt // insert_id // insert_singleton_op_empty.
-        do 2 rewrite right_id_L.
-        iCombine "Hown_frag Hown_emp" as "Hown_frag".
-        rewrite Qp.div_2.
-
-        iPoseProof ("Himp" $! vs val with "[Hpt Hnode]") as "Hlist".
-        { iNext; by iFrame. }
-        rewrite /opt_map/opt_insert insert_id //.
-
-        iMod ("Hclose" with "[Hlist Hown_auth Hown_toks Hown_frac]") as "_".
-        { iNext; iExists M', S', L; by iFrame "# ∗". }
-        iModIntro; iApply ("HΦ" $! val).
-        destruct (decide (t < val_ts val)); last done.
-        by iFrame "# ∗".
-      + wp_alloc v' as "Hval'".
-        iMod (mapsto_persist with "Hval'") as "#Hval'".
-        wp_pures. wp_lam. wp_pures.
-        set (val' := (v, t, v')); rewrite (fold_rep_to_val val').
-
-        iInv (levelN 0) as (M' S' L) "(Hinv_sub & >Hown_frac & >%Hequiv)" "Hclose".
-        iDestruct "Hinv_sub" as "(>%Hperm & >%Hsort & >Hown_auth & >Hown_toks & Hlist)".
-
-        iAssert ⌜ In node L ⌝%I with "[Hown_auth]" as %Hin.
-        {
-          iDestruct (own_valid_2 with "Hown_auth Hown_succ") 
-            as %[Hvalid%gset_included]%auth_both_valid_discrete.
-          rewrite -elem_of_list_In Hperm elem_of_elements.
-          iPureIntro; set_solver.
-        }
-
-        rewrite list_equiv_invert_L; last done.
-        iDestruct "Hlist" as (val'' γ l s succ) "(_ & Hpt & _ & _ & _ & >Hnode & >%Hval & Himp)".
-        iDestruct (mapsto_agree with "Hval Hnode") as %<-%rep_to_val_inj.
-        destruct Hval as [vs [Hsome Hv]].
-
-        assert (M ⋅ ∅ = M) as <- by rewrite right_id_L //.
-        rewrite -(Qp.div_2 q) frac_auth_frag_op.
-        iDestruct "Hown_frag" as "(Hown_frag & Hown_emp)".
-        iMod (own_update_2 with "Hown_frac Hown_emp") as "[Hown_frac Hown_emp]".
-        { 
-          apply frac_auth_update. 
-          apply (insert_alloc_local_update _ _ 
-            (node_key node) 
-            (prodZ vs (val_ts val)) 
-            (prodZ {[v]} t ⋅ prodZ vs (val_ts val)) 
-            (prodZ {[v]} t)
-          ); auto.
-          apply arg_max_local_update.
-        }
-
-        rewrite insert_singleton_op_Some // insert_singleton_op_empty.
-        do 2 rewrite right_id_L.
-        iCombine "Hown_frag Hown_emp" as "Hown_frag".
-        rewrite Qp.div_2.
-
-        iCombine "Hval Hnode" as "Hval"; wp_store.
-        iDestruct "Hval" as "(Hval & Hnode)".
-
-        set (p := prodZ {[ v ]} t ⋅ prodZ vs (val_ts val)).
-        iPoseProof ("Himp" $! (args p) val' with "[Hpt Hnode]") as "Hlist".
-        { 
-          iFrame; iPureIntro; unfold val_v, p; simpl.
-          destruct (decide (t = val_ts val)) as [<-|].
-          + rewrite arg_max_eq /args.
-            by apply elem_of_union_l, elem_of_singleton.
-          + rewrite comm_L arg_max_lt /args ?elem_of_singleton //; lia.
-        }
-        rewrite /opt_map/opt_insert.
-
-        assert (prodZ (args p) (val_ts val') = p) as ->.
-        { 
-          unfold p; destruct (decide (t = val_ts val)) as [<-|].
-          + rewrite arg_max_eq //.
-          + rewrite comm_L arg_max_lt //; lia.
-        }
-
-        rewrite insert_singleton_op_Some_L //.
-        rewrite -(dom_singleton_op_Some _ (node_key node) (prodZ {[v]} t)) // in Hequiv.
-
-        iMod ("Hclose" with "[Hlist Hown_auth Hown_toks Hown_frac]") as "_".
-        { iNext; iExists ({[node_key node := prodZ {[v]} t]} ⋅ M'), S', L; by iFrame "# ∗". }
-        iModIntro; iApply ("HΦ" $! val').
-        destruct (decide (t < val_ts val)); first done.
-        by iFrame "# ∗".
-    Qed.
-
-    Theorem tryInsert_spec (k v t h: Z) (head curr: node_rep) 
-      (M: gmap Z (argmax Z)) (q: frac)
-      (bot: bot_gname) (Γ: sub_gname) :
-      INT_MIN < k < INT_MAX →
-      {{{
-        inv (levelN 0) (lazy_list_inv 0 head (Some bot) Γ None)
-        ∗
-        own (s_frac bot) (◯F{q} M)
-        ∗
-        (⌜ curr = head ⌝ ∨ own (s_auth Γ) (◯ {[ curr ]}))
-        ∗
-        ⌜ node_key curr < k ⌝
-        ∗
-        ⌜ 0 ≤ h ⌝ 
-      }}}
-        tryInsert (rep_to_node curr) #k #v #t #h
-      {{{ (opt: val) (n: loc) (new: node_rep), RET opt;
-        own (s_frac bot) (◯F{q} (M ⋅ {[ k := prodZ {[ v ]} t ]}))
-        ∗
-        ( 
-          ⌜ opt = NONEV ⌝ ∨ 
-          ( 
-            ⌜ opt = SOMEV #n ⌝ 
-            ∗ 
-            own (s_auth Γ) (◯ {[ new ]})
-            ∗ 
-            own (s_toks Γ) (◯ GSet {[ node_key new ]})
-            ∗ 
-            ⌜ node_key new = k ⌝
-            ∗
-            n ↦□ rep_to_node new
-            ∗
-            (node_next new +ₗ 1) ↦∗ replicate (Z.to_nat h) #()
-            ∗
-            (node_locks new +ₗ 1) ↦∗ replicate (Z.to_nat h) #()
-          )
-        )
-      }}}.
-    Proof.
-      iIntros (Hkey_range Φ) "(#Hinv & Hown_frag & #Hown_curr & %Hrange & %Hh) HΦ".
-      wp_lam. wp_pures.
-
-      wp_apply findLock_spec.
-      { iFrame "#". iPureIntro; lia. }
-      iIntros (pred succ) "(%Hrange' & #Hown_pred & #Hown_succ & Hlock)".
-      iDestruct "Hlock" as (γ l s) "(#Hl & #Hlock & Hnext & #Hs & Hval & Hlocked)".
-      do 2 rewrite loc_add_0.
-
-      wp_pures. wp_lam. wp_pures. wp_load. 
-      wp_pures. wp_lam. wp_pures.
-      case_bool_decide as Hcase; wp_if.
-      + assert (k = node_key succ) as Heq by congruence.
-        iDestruct "Hown_succ" as "[Hown_succ|%Hsucc]"; last first.
-        { subst; exfalso. rewrite /node_key/tail/= in Hkey_range; lia. }
-        
-        iDestruct "Hval" as (succ') "(#Hs' & Hval)".
-        iDestruct (mapsto_agree with "Hs Hs'") as %<-%rep_to_node_inj.
-        iDestruct "Hval" as "[%Htail|Hval]".
-        { subst; exfalso. rewrite /node_key/tail/= in Hkey_range; lia. }
-        iDestruct "Hval" as (val) "Hval".
-
-        wp_apply (update_spec with "[$]").
-        iIntros (val') "(Hown_frag & Hval & _)".
-        wp_pures.
-
-        wp_apply (release_spec with "[Hnext Hval Hlocked]").
-        {
-          iFrame "# ∗";  iExists s; rewrite loc_add_0. 
-          iFrame; iExists succ. 
-          iFrame "#"; iRight; by iExists val'.
-        }
-        iIntros "_". wp_pures.
-        iModIntro; iApply "HΦ".
-        rewrite -Heq. iFrame "# ∗". by iLeft.
-      + assert (k ≠ node_key succ) as Hneq by congruence.
-
-        wp_apply (createAndLink_spec with "[Hnext Hval Hown_frag]").
-        { done. }
-        { iFrame "# ∗". iPureIntro; lia. }
-        iIntros (n new) "(Hown_map & Hown_frag & Hown_tok & Hkey & Hnext & #Hn & Hval & Hnexts & Hlocks)".
-        wp_let.
-
-        wp_apply (release_spec with "[Hnext Hval Hlocked]").
-        { 
-          iFrame "# ∗";  iExists n; rewrite loc_add_0. 
-          iFrame; iExists new. 
-          iFrame "#"; iRight; by iExists (v, t, dummy_null).
-        }
-        iIntros "_"; wp_pures.
-        iModIntro; iApply ("HΦ" $! _ n new).
-        iFrame "# ∗". iRight; by iFrame.
-    Qed.
-
-    Theorem insert_spec (lvl: Z) (head curr new: node_rep) 
-      (Γ γ: sub_gname) (n: loc) :
-      INT_MIN < node_key new < INT_MAX →
-      {{{
-        inv (levelN lvl) (lazy_list_inv lvl head None Γ (Some γ))
-        ∗
-        (⌜ curr = head ⌝ ∨ own (s_auth Γ) (◯ {[ curr ]}))
-        ∗
-        ⌜ node_key curr < node_key new ⌝
-        ∗ 
-        own (s_auth γ) (◯ {[ new ]})
-        ∗ 
-        own (s_toks γ) (◯ GSet {[ node_key new ]})
-        ∗
-        n ↦□ rep_to_node new
-        ∗
-        (node_next new +ₗ lvl) ↦ #()
-        ∗
-        (node_locks new +ₗ lvl) ↦ #()
-      }}}
-        insert (rep_to_node curr) #lvl #n
-      {{{ RET #();
-        own (s_auth Γ) (◯ {[ new ]})
-        ∗ 
-        own (s_toks Γ) (◯ GSet {[ node_key new ]})
-      }}}.
-    Proof.
-      iIntros (Hkey_range Φ) "(#Hinv & #Hown_curr & %Hrange & Hown_frag & Hown_tok & #Hn & Hnext & Hlocks) HΦ".
-      wp_lam. wp_let. wp_let.
-      wp_load. wp_lam. wp_pures.
-
-      wp_apply findLock_spec.
-      { iFrame "#". iPureIntro; lia. }
-      iIntros (pred succ) "(%Hrange' & #Hown_pred & #Hown_succ & Hlock)".
-      iDestruct "Hlock" as (γl l s) "(#Hl & #Hlock & Hnext' & #Hs & _ & Hlocked)".
-      wp_pures. wp_lam. wp_pures.
-
-      wp_bind (Load _).
-      iInv (levelN lvl) as (M' S' L) "(Hinv_sub & _)" "Hclose".
-      iDestruct "Hinv_sub" as "(>%Hperm & >%Hsort & >Hown_auth & >Hown_toks & Hlist)".
-      wp_load.
-
-      iAssert ⌜ node_key new ≠ node_key succ ⌝%I
-        with "[Hown_auth Hown_succ Hown_tok Hlist]" as %Hneq.
+      iAssert ⌜ node_key new ≠ node_key succ ⌝%I as %Hneq.
       {
-        iDestruct "Hown_succ" as "[Hown|%Heq]"; last first.
-        { iPureIntro; rewrite Heq /tail/node_key/=; rewrite /node_key in Hkey_range; lia. } 
-
-        iDestruct (own_valid_2 with "Hown_auth Hown") 
+        iDestruct "Hsucc" as "[->|Hsucc]"; first (iPureIntro;
+          rewrite /tail{2}/node_key/=; rewrite /tail{4}/node_key/= in Hk''; lia). 
+        iDestruct (own_valid_2 with "Hauth Hsucc") 
           as %[Hvalid%gset_included]%auth_both_valid_discrete.
-
-        assert (In succ L).
-        { rewrite -elem_of_list_In Hperm elem_of_elements. set_solver. }
-
-        rewrite list_equiv_invert_L; last done.
-        iDestruct "Hlist" as (? ? ? ? ?) "(_ & _ & _ & _ & _ & Hnode & _)".
-        iDestruct "Hnode" as "(_ & Hown_tok')".
-
-        iDestruct (own_valid_2 with "Hown_tok Hown_tok'") as 
+        rewrite (big_sepS_delete (has_sub _) _ succ); last set_solver.
+        iDestruct "Hsubs" as "[[Hfrag Htok] Hsubs]".
+        iDestruct (own_valid_2 with "Htok Htok'") as 
           %Hdisj%auth_frag_op_valid_1%gset_disj_valid_op.
         iPureIntro; set_solver.
       }
 
-      iMod ("Hclose" with "[Hlist Hown_auth Hown_toks]") as "_".
-      { iNext; iExists M', S', L; by iFrame "# ∗". }
-      iModIntro; wp_pures.
+      rewrite (big_sepS_delete (has_next _ _) _ pred) //.
+      iDestruct "Hnexts" as "[Hnext Hnexts]".
+      iDestruct "Hnext" as (s' succ') "(Hnext & #Hs' & _ & Hkeys)".
+      iDestruct (mapsto_agree with "Hpt Hnext") as %Hs; 
+        symmetry in Hs; inversion Hs; subst; clear Hs.
+      iDestruct (mapsto_agree with "Hs Hs'") as %<-%rep_to_node_inj.
+      iClear "Hs'"; iCombine "Hpt Hnext" as "Hpt".
+      wp_store. iDestruct "Hpt" as "[Hpt Hnext]".
 
-      wp_apply (link_spec with "[Hnext' Hown_frag Hown_tok Hnext Hlocks]").
-      { done. }
-      { iFrame "# ∗". iPureIntro; lia. }
-      iIntros "(Hown_frag & Hown_tok & Hnext)".
+      iMod (own_update with "Hauth") as "[Hauth Hfrag]".
+      { by apply auth_update_alloc, (op_local_update_discrete _ _ {[new]}). }
+      rewrite right_id (comm_L _ {[new]}). iDestruct "Hfrag" as "#Hfrag".
 
-      wp_pures.
-      wp_apply (release_spec with "[Hnext Hlocked]").
-      { iFrame "# ∗"; iExists n; iFrame. }
-      iIntros "_"; iApply "HΦ"; iFrame.
-      Unshelve. done.
+      rewrite (ZRange_split (node_key new)); last lia.
+      iDestruct "Hkeys" as "((Hkeys & Hkey) & Hkeys')".
+      iDestruct (own_valid_2 with "Hdisj Hkey") as %Hdisj%gset_disj_valid_op.
+      iCombine "Hdisj Hkey" as "Hdisj"; rewrite gset_disj_union //.
+
+      iMod (own_update with "Htoks") as "[Htoks Htok]".
+      { by apply auth_update_alloc, (gset_disj_alloc_op_local_update _ _ {[ node_key new ]}). }
+      rewrite ?gset_disj_union // right_id_L (comm_L _ {[ node_key new ]}).
+
+      iMod ("Hclose" with "[- Hpt Htok Hlocked]") as "AP".
+      { 
+        rewrite /lazy_list set_map_union_L set_map_singleton_L; iFrame.
+        assert (node_key new ≠ node_key head) by lia.
+        iSplitL "Hnexts Hnext Hnew Hfrag Hkeys Hkeys'"; 
+          last iSplitL "Hlocks Hlock Hnew'".
+        + rewrite assoc_L (comm_L _ _ {[new]}).
+          iApply big_sepS_insert; first set_solver.
+          iSplitL "Hnew Hkeys'"; first (iExists s, succ; iFrame "# ∗").
+          iApply big_sepS_delete; first done.
+          iFrame. iExists n, new; iFrame "# ∗".
+        + rewrite assoc_L (comm_L _ _ {[new]}).
+          iApply big_sepS_insert; first set_solver.
+          iFrame. iExists (node_lock new +ₗ lvl), false.
+          rewrite -Qp.quarter_three_quarter; iDestruct "Hlock" as "[? ?]".
+          rewrite Qp.quarter_three_quarter.
+          iFrame. iSplit; first done. iExists s; iFrame.
+          by unfold locked_val; case_decide; first lia.
+        + rewrite comm_L big_sepS_insert; last set_solver. iFrame.
+      }
+      iModIntro. wp_pures.
+
+      clear dependent S.
+      iAssert (in_lock lvl pred)%I with "[Hpt]" as "Hin_lock". 
+      { iExists n; iFrame "Hpt". by unfold locked_val; case_decide; first lia. }
+      awp_apply (release_spec with "Hlocked Hin_lock").
+      iApply (aacc_apst_sub with "[] AP"); try done.
+      { iIntros "!> %S"; by iApply node_has_lock. }
+      iIntros (S) "Hlazy".
+      iDestruct (node_has_lock with "Hpred Hlazy") as "[Hlock Hlazy]".
+      iAaccIntro with "Hlock".
+      { iIntros "H"; iDestruct ("Hlazy" with "H") as "?"; iModIntro; iFrame; by iIntros. }
+      iIntros "Hlock"; iModIntro; iFrame "Hlock".
+      iIntros "Hlock"; iDestruct ("Hlazy" with "Hlock") as "Hlazy".
+      iFrame "Hlazy". iIntros "AP". rewrite difference_empty_L.
+      iMod (atomic_post_commit with "AP") as "HΦ".
+      iModIntro. iIntros "_".
+      iApply "HΦ". iFrame "# ∗".
     Qed.
 
+    Theorem tryInsert_spec (k v t h: Z) (head curr: node_rep) (Γ: lazy_gname) :
+      node_key head < k < INT_MAX →
+      node_key curr < k →
+      0 ≤ h →
+      (⌜ curr = head ⌝ ∨ own Γ.(auth_gname) (◯ {[ curr ]})) -∗
+      <<< ∀∀ S m, jf_map head S m Γ >>>
+        tryInsert (rep_to_node curr) #k #v #t #h @ ∅
+      <<< ∃∃ opt node,
+        jf_map head (case_set S node m k) (case_map m k v t) Γ,
+      RET opt >>>
+      {{{
+        match m !! k with 
+        | None => ∃ (n: loc),
+                    ⌜ opt = SOMEV #n ⌝
+                    ∗
+                    n ↦□ rep_to_node node
+                    ∗ 
+                    ⌜ node_key node = k ⌝
+                    ∗
+                    (node_next node +ₗ 1) ↦∗ replicate (Z.to_nat h) #()
+                    ∗
+                    (node_lock node +ₗ 1) ↦∗ replicate (Z.to_nat h) #false
+                    ∗
+                    has_sub Γ node
+        | Some _ => ⌜ opt = NONEV ⌝
+        end
+      }}}.
+    Proof.
+      iIntros "%Hk %Hk' %Hh #Hcurr %Φ AU".
+      wp_lam; wp_pures.
+
+      awp_apply (findLock_spec with "Hcurr"); first lia.
+      iApply (aacc_aupd_sub with "[] AU"); try done.
+      { iIntros "!> %S %m [H Hmap]". iExists S. iFrame "H". iIntros. iFrame. }
+      iIntros (S m) "[Hlazy Hmap]"; iAaccIntro with "Hlazy".
+      { iIntros; iModIntro; iFrame; by iIntros. }
+      iIntros (pred succ) "[Hlazy %Hnin]".
+      iModIntro. iExists S. iFrame "Hlazy". iIntros "Hlazy".
+      iLeft. iFrame "Hlazy Hmap". iIntros "AU". clear dependent S m.
+      iModIntro. iIntros "(#Hpred & #Hsucc & %Hk'' & Hlocked)".
+      iDestruct "Hlocked" as (s) "(Hpt & #Hs & Hval & Hlocked)".
+      iDestruct "Hval" as (?) "[Hs' Hsucc']".
+      iDestruct (mapsto_agree with "Hs Hs'") as %<-%rep_to_node_inj; iClear "Hs'".
+      iModIntro. wp_pures; wp_lam; wp_pures; wp_lam; wp_pures.
+
+      case_bool_decide as Hcase; wp_if.
+      + assert (k = node_key succ) as Heq by congruence.
+        iDestruct "Hsucc" as "[->|Hsucc]".
+        { rewrite /node_key/tail/= in Heq; lia. }
+        iDestruct "Hsucc'" as "[->|Hsucc']".
+        { rewrite /node_key/tail/= in Heq; lia. }
+        iDestruct "Hsucc'" as (val) "Hvpt".
+        wp_lam; wp_pures.
+
+        (* We start the case analysis here, since it's easier to use the load
+        operation as the linearisation point for when no update occurs. *)
+        destruct (decide (t < (val_vt val).2)) as [Ht|Ht].
+        - (* The key already exists with a more recent timestamp*)
+          wp_bind (Load _). iMod "AU" as (S m) "[[Hlazy Hmap] [_ Hclose]]".
+          iDestruct "Hlazy" as "(Hauth & Hdisj & Htoks & Hnexts & Hlocks & _)".
+          iDestruct (own_valid_2 with "Hauth Hsucc") 
+            as %[?%gset_included]%auth_both_valid_discrete.
+          iDestruct "Hmap" as (γ) "(%Hdom & Hgmap & Hvals)".
+          rewrite (big_sepS_delete (has_val _) _ succ); last set_solver.
+          iDestruct "Hvals" as "[Hval Hvals]".
+          iDestruct "Hval" as (? vl) "(Hvpt' & Hkey & Hvl)".
+          iDestruct (ghost_map_lookup with "Hgmap Hkey") as %Hsome; 
+            rewrite -Heq in Hsome.
+          iDestruct (mapsto_agree with "Hvpt Hvpt'") as %<-%rep_to_val_inj.
+
+          wp_load. rewrite /case_set /case_map Hsome.
+          case_decide as Hcase'; simpl in Hcase'; last lia.
+          iMod ("Hclose" $! NONEV succ with "[- Hpt Hvpt Hlocked]") as "AP".
+          {
+            iFrame. iExists γ. iFrame "Hgmap". iSplit; first done.
+            iApply (big_sepS_delete _ _ succ); first set_solver.
+            iFrame "Hvals". iExists val, vl. iFrame.
+          }
+          iModIntro. wp_pures; wp_lam; wp_pures.
+          case_bool_decide as Ht'; wp_if; last first.
+          { unfold val_vt in Ht; unfold val_t in Ht'; lia. }
+
+          clear dependent S m γ vl.
+          iAssert (in_lock 0 pred)%I with "[Hpt Hvpt]" as "Hin_lock". 
+          { iExists s; iFrame "Hpt". iExists succ; iFrame "Hs". iRight; by iExists val. }
+          rewrite loc_add_0; awp_apply (release_spec with "Hlocked Hin_lock").
+          iApply (aacc_apst_sub with "[] AP"); try done.
+          { 
+            iIntros "!> %S %m [Hlazy Hmap]". 
+            iDestruct (node_has_lock with "Hpred Hlazy") as "[Hlock Hlazy]".
+            unfold has_lock; rewrite loc_add_0. by iFrame.
+          }
+          iIntros (S m) "[Hlazy Hmap]".
+          iDestruct (node_has_lock with "Hpred Hlazy") as "[Hlock Hlazy]".
+          unfold has_lock; rewrite loc_add_0.
+          iAaccIntro with "Hlock".
+          { iIntros "H"; iDestruct ("Hlazy" with "H") as "?"; iModIntro; iFrame; by iIntros. }
+          iIntros "Hlock"; iModIntro; iFrame "Hlock".
+          iIntros "Hlock"; iDestruct ("Hlazy" with "Hlock") as "Hlazy".
+          iFrame "Hlazy Hmap". iIntros "AP". rewrite difference_empty_L.
+          iMod (atomic_post_commit with "AP") as "HΦ".
+          iModIntro. iIntros "_". iModIntro. wp_pures. by iApply "HΦ".
+        - (* The key already exists but with an outdated timestamp *)
+          wp_load. wp_pures; wp_lam; wp_pures.
+          case_bool_decide as Ht'; wp_if.
+          { unfold val_vt in Ht; unfold val_t in Ht'; lia. }
+
+          wp_alloc prev as "Hprev". wp_pures; wp_lam; wp_pures.
+          iMod (mapsto_persist with "Hprev") as "#Hprev".
+          set (val' := (v, t, prev)).
+          rewrite (fold_rep_to_val val').
+
+          wp_bind (Store _ _). iMod "AU" as (S m) "[[Hlazy Hmap] [_ Hclose]]".
+          iDestruct "Hlazy" as "(Hauth & Hdisj & Htoks & Hnexts & Hlocks & _)".
+          iDestruct (own_valid_2 with "Hauth Hsucc") 
+            as %[?%gset_included]%auth_both_valid_discrete.
+          iDestruct "Hmap" as (γ) "(%Hdom & Hgmap & Hvals)".
+          rewrite (big_sepS_delete (has_val _) _ succ); last set_solver.
+          iDestruct "Hvals" as "[Hval Hvals]".
+          iDestruct "Hval" as (? vl) "(Hvpt' & Hkey & Hvl)".
+          iDestruct (ghost_map_lookup with "Hgmap Hkey") as %Hsome; 
+            rewrite -Heq in Hsome.
+          iDestruct (mapsto_agree with "Hvpt Hvpt'") as %<-%rep_to_val_inj.
+          iCombine "Hvpt Hvpt'" as "Hvpt". wp_store.
+          iDestruct "Hvpt" as "[Hvpt Hvpt']".
+
+          iMod (ghost_map_update (v, t, val_vt val :: vl) with "Hgmap Hkey")
+            as "[Hgmap Hkey]".
+
+          rewrite /case_set /case_map Hsome Heq.
+          case_decide as Hcase'; simpl in Hcase'; first lia.
+          iMod ("Hclose" $! NONEV succ with "[- Hpt Hvpt Hlocked]") as "AP".
+          {
+            iFrame. iExists γ. iFrame "Hgmap". iSplit; 
+              first rewrite -Heq -Hdom dom_insert_lookup_L //.
+            iApply (big_sepS_delete _ _ succ); first set_solver.
+            iFrame "Hvals". iExists val', (val_vt val :: vl). iFrame.
+            iExists (val_p val); iFrame "# ∗".
+          }
+          iModIntro. wp_pures.
+
+          clear dependent S m γ vl.
+          iAssert (in_lock 0 pred)%I with "[Hpt Hvpt]" as "Hin_lock". 
+          { iExists s; iFrame "Hpt". iExists succ; iFrame "Hs". iRight; by iExists val'. }
+          rewrite loc_add_0; awp_apply (release_spec with "Hlocked Hin_lock").
+          iApply (aacc_apst_sub with "[] AP"); try done.
+          { 
+            iIntros "!> %S %m [Hlazy Hmap]". 
+            iDestruct (node_has_lock with "Hpred Hlazy") as "[Hlock Hlazy]".
+            unfold has_lock; rewrite loc_add_0. by iFrame.
+          }
+          iIntros (S m) "[Hlazy Hmap]".
+          iDestruct (node_has_lock with "Hpred Hlazy") as "[Hlock Hlazy]".
+          unfold has_lock; rewrite loc_add_0.
+          iAaccIntro with "Hlock".
+          { iIntros "H"; iDestruct ("Hlazy" with "H") as "?"; iModIntro; iFrame; by iIntros. }
+          iIntros "Hlock"; iModIntro; iFrame "Hlock".
+          iIntros "Hlock"; iDestruct ("Hlazy" with "Hlock") as "Hlazy".
+          iFrame "Hlazy Hmap". iIntros "AP". rewrite difference_empty_L.
+          iMod (atomic_post_commit with "AP") as "HΦ".
+          iModIntro. iIntros "_". iModIntro. wp_pures. by iApply "HΦ".
+      + (* The key does not exists in the map *)
+        assert (k ≠ node_key succ) by congruence.
+        
+        wp_alloc next as "Hnexts"; first lia. wp_let.
+        wp_alloc lock as "Hlocks"; first lia. wp_let.
+        assert (Z.to_nat (h + 1) = S (Z.to_nat h)) as -> by lia.
+        rewrite ?replicate_S ?array_cons ?loc_add_0.
+        iDestruct "Hnexts" as "[Hnext Hns]".
+        iDestruct "Hlocks" as "[Hlock Hls]".
+
+        wp_alloc vpt as "[Hvpt Hvpt']". wp_let.
+        wp_alloc n as "Hn". iMod (mapsto_persist with "Hn") as "#Hn". wp_let.
+        set (val := (v, t, dummy_null)); set (new := (k, vpt, next, lock)).
+        rewrite (fold_rep_to_val val) (fold_rep_to_node new).
+
+        wp_lam; wp_pures. wp_load. wp_load. wp_lam; wp_pures.
+        wp_store. iDestruct "Hnext" as "[Hnext Hnext']".
+        wp_lam; wp_pures.
+
+        wp_bind (Store _ _). iMod "AU" as (S m) "[[Hlazy Hmap] [_ Hclose]]".
+        iDestruct (singleton_frag_in with "Hpred Hlazy") as %Hpred.
+        iDestruct "Hlazy" as "(Hauth & Hdisj & Htoks & Hnexts & Hlocks & _)".
+
+        rewrite (big_sepS_delete (has_next _ _) _ pred) //.
+        iDestruct "Hnexts" as "[Hpt' Hnexts]".
+        iDestruct "Hpt'" as (s' succ') "(Hpt' & #Hs' & _ & Hkeys)".
+        rewrite loc_add_0.
+        iDestruct (mapsto_agree with "Hpt Hpt'") as %Hs; 
+          symmetry in Hs; inversion Hs; subst; clear Hs.
+        iDestruct (mapsto_agree with "Hs Hs'") as %<-%rep_to_node_inj; iClear "Hs'".
+        iCombine "Hpt Hpt'" as "Hpt".
+        wp_store. iDestruct "Hpt" as "[Hpt Hpt']".
+
+        iMod (own_update with "Hauth") as "[Hauth Hfrag]".
+        { by apply auth_update_alloc, (op_local_update_discrete _ _ {[new]}). }
+        rewrite right_id (comm_L _ {[new]}). iDestruct "Hfrag" as "#Hfrag".
+
+        rewrite (ZRange_split (node_key new)); last first.
+        { replace (node_key new) with k by auto; lia. }
+        iDestruct "Hkeys" as "((Hkeys & Hkey) & Hkeys')".
+        iDestruct (own_valid_2 with "Hdisj Hkey") as %Hdisj%gset_disj_valid_op.
+        iCombine "Hdisj Hkey" as "Hdisj"; rewrite gset_disj_union //.
+
+        iMod (own_update with "Htoks") as "[Htoks Htok]".
+        { by apply auth_update_alloc, (gset_disj_alloc_op_local_update _ _ {[ node_key new ]}). }
+        rewrite ?gset_disj_union // right_id_L (comm_L _ {[ node_key new ]}).
+
+        iDestruct "Hmap" as (γ) "(%Hdom & Hgmap & Hvals)".
+        assert (m !! k = None) as Heq by (rewrite -not_elem_of_dom; set_solver).
+        iMod (ghost_map_insert k (v, t, nil) with "Hgmap") as "[Hgmap Hval]"; 
+          first done; rewrite /case_set /case_map Heq; clear Heq.
+
+        rewrite -(loc_add_0 (node_next pred)) -(loc_add_0 (node_next new)).
+        iMod ("Hclose" $! (SOMEV #n) new with "[- Hpt Hvpt Hlocked Hns Hls Htok]") as "AP".
+        {
+          iSplitR "Hvals Hvpt' Hgmap Hval".
+          + rewrite /lazy_list set_map_union_L set_map_singleton_L; iFrame.
+            assert (k ≠ node_key head) by lia.
+            iSplitR "Hlock Hlocks Hnext' Hsucc'"; last (iSplit; last done).
+            - rewrite assoc_L (comm_L _ ({[head]} ∪ S)).
+              iApply big_sepS_insert; first set_solver.
+              iSplitL "Hnext Hkeys'"; first (iExists s, succ; iFrame "# ∗").
+              iApply big_sepS_delete; first done.
+              iFrame "Hnexts". iExists n, new; iFrame "# ∗".
+            - rewrite assoc_L (comm_L _ ({[head]} ∪ S)).
+              iApply big_sepS_insert; first set_solver.
+              iFrame "Hlocks". iExists (node_lock new), false.
+              rewrite -Qp.quarter_three_quarter; iDestruct "Hlock" as "[? ?]".
+              rewrite Qp.quarter_three_quarter.
+              iFrame. iSplitL ""; first rewrite loc_add_0 //. 
+              iExists s; iFrame. iExists succ; iFrame "# ∗".
+          + iExists γ. iFrame "Hgmap". iSplit; first iPureIntro.
+            - rewrite set_map_union_L set_map_singleton_L -Hdom dom_insert_L comm_L //.
+            - rewrite comm_L; iApply big_sepS_insert; first set_solver.
+              iFrame "Hvals". iExists val, nil. by iFrame.
+        }
+        iModIntro. wp_pures.
+
+        clear dependent S m γ.
+        iAssert (in_lock 0 pred)%I with "[Hpt Hvpt]" as "Hin_lock". 
+        { iExists n; iFrame "Hpt". iExists new. iFrame "Hn". iRight. by iExists val. }
+        awp_apply (release_spec with "Hlocked Hin_lock").
+        iApply (aacc_apst_sub with "[] AP"); try done.
+        {
+          iIntros "!> %S %m [Hlazy Hmap]". 
+          iDestruct (node_has_lock with "Hpred Hlazy") as "[Hlock Hlazy]".
+          unfold has_lock; rewrite loc_add_0. by iFrame.
+        }
+        iIntros (S m) "[Hlazy Hmap]".
+        iDestruct (node_has_lock with "Hpred Hlazy") as "[Hlock Hlazy]".
+        unfold has_lock; rewrite loc_add_0.
+        iAaccIntro with "Hlock".
+        { iIntros "H"; iDestruct ("Hlazy" with "H") as "?"; iModIntro; iFrame; by iIntros. }
+        iIntros "Hlock"; iModIntro; iFrame "Hlock".
+        iIntros "Hlock"; iDestruct ("Hlazy" with "Hlock") as "Hlazy".
+        iFrame "Hlazy Hmap". iIntros "AP". rewrite difference_empty_L.
+        iMod (atomic_post_commit with "AP") as "HΦ".
+        iModIntro. iIntros "_". iModIntro. wp_pures.
+        iApply "HΦ". iExists n. by iFrame "# ∗".
+    Qed.
   End Proofs.
 End InsertSpec.
