lazy_list/code.v
@@ -1,23 +1,24 @@
-From iris.heap_lang Require Export notation spin_lock.
+From SkipList.atomic Require Import proofmode lock.
+
+From iris.heap_lang Require Import notation.
 
 
 Section node_rep.
-  Definition node_rep : Type := Z * loc * val.
+  Definition node_rep : Type := Z * loc * loc.
   Definition dummy_null : loc := {|loc_car := 0|}.
-  Definition dummy_lock : val := #().
 
   Definition node_key (n: node_rep) : Z := n.1.1.
   Definition node_next (n: node_rep) : loc := n.1.2.
-  Definition node_lock (n: node_rep) : val := n.2.
+  Definition node_lock (n: node_rep) : loc := n.2.
 
   Definition nodeKey : val := λ: "l", Fst (Fst "l").
   Definition nodeNext : val := λ: "l", Snd (Fst "l").
   Definition nodeLock : val := λ: "l", Snd "l".
 
   Definition rep_to_node (n: node_rep) : val :=
-    (#(node_key n), #(node_next n), (node_lock n)).
+    (#(node_key n), #(node_next n), #(node_lock n)).
   Lemma fold_rep_to_node (n: node_rep) :
-    ((#(node_key n), #(node_next n), (node_lock n)))%V = rep_to_node n.
+    ((#(node_key n), #(node_next n), #(node_lock n)))%V = rep_to_node n.
   Proof. done. Qed.
   Lemma rep_to_node_inj rep rep':
     rep_to_node rep = rep_to_node rep' → rep = rep'.
@@ -37,12 +38,13 @@ End LAZY_LIST_PARAMS.
 Module LazyList (Params: LAZY_LIST_PARAMS).
   Import Params.
   
-  Definition tail : node_rep := (INT_MAX, dummy_null, dummy_lock).  
+  Definition tail : node_rep := (INT_MAX, dummy_null, dummy_null).
 
   Definition new : val := 
     λ: "_", 
-      let: "t" := ref (rep_to_node tail) in
-        ref (#INT_MIN, "t", newlock #()).
+      let: "n" := ref (rep_to_node tail) in
+      let: "l" := ref #false in
+        ref (#INT_MIN, "n", "l").
 
   Definition find : val := 
     rec: "find" "pred" "k" :=
@@ -76,8 +78,9 @@ Module LazyList (Params: LAZY_LIST_PARAMS).
         if: "k" = nodeKey "succ"
         then release "lock"
         else let: "np" := nodeNext "pred" in
-             let: "next" := ref !"np" in
-               "np" <- ("k", "next", newlock #());;
+             let: "n" := ref !"np" in
+             let: "l" := ref #false in
+               "np" <- ("k", "n", "l");;
                release "lock".
 
 End LazyList.
