atomic/lock.v
@@ -1,0 +1,105 @@
+From SkipList.atomic Require Import weakestpre proofmode.
+
+From iris.heap_lang Require Import notation.
+Import derived_laws_later.bi.
+
+
+Definition newlock : val := λ: <>, ref #false.
+Definition try_acquire : val := λ: "l", CAS "l" #false #true.
+Definition acquire : val :=
+  rec: "acquire" "l" := if: try_acquire "l" then #() else "acquire" "l".
+Definition release : val := λ: "l", "l" <- #false.
+
+Section proof.
+  Context `{!heapGS Σ}.
+
+  Definition locked (lk: val) : iProp Σ :=
+    ∃ (l: loc), ⌜ lk = #l ⌝ ∗ l ↦{#3 / 4} #true.
+
+  Definition is_lock (lk: val) (R: iProp Σ) : iProp Σ := 
+    ∃ (l: loc) (b: bool), ⌜ lk = #l ⌝ ∗ l ↦{#1 / 4} #b ∗ 
+      if b then True else l ↦{#3 / 4} #false ∗ R.
+
+  Global Instance is_lock_timeless lk R `{!Timeless R} : Timeless (is_lock lk R).
+  Proof.
+    do 2 (apply exist_timeless; intros ?).
+    do 2 (apply sep_timeless; first apply _).
+    case_match; last apply sep_timeless; apply _.
+  Qed.
+
+  Lemma newlock_spec (R : iProp Σ) :
+    {{{ R }}} newlock #() {{{ lk, RET lk; is_lock lk R }}}.
+  Proof.
+    iIntros (Φ) "HR HΦ". wp_lam. wp_alloc l as "Hl".
+    rewrite -Qp.quarter_three_quarter; iDestruct "Hl" as "(Hl1 & Hl2)".
+    iModIntro; iApply "HΦ". iExists l, false. by iFrame.
+  Qed.
+
+  Lemma try_acquire_spec (lk: val) (R : iProp Σ) :
+    ⊢ <<< is_lock lk R >>> try_acquire lk @ ∅
+    <<< ∃∃ b, is_lock lk R, RET #b >>>
+    {{{ if b is true then locked lk ∗ R else True }}}.
+  Proof.
+    iIntros (Φ) "AU"; rewrite difference_empty_L.
+    wp_lam. wp_bind (CmpXchg _ _ _).
+    iMod "AU" as "[Hlock [_ Hclose]]".
+    iDestruct "Hlock" as (l []) "(-> & Hl & Hif)".
+    + wp_cmpxchg_fail.
+      iDestruct ("Hclose" $! false with "[Hl Hif]") as ">AP".
+      { iFrame. iExists l, true. by iFrame. }
+      iMod (atomic_post_commit with "AP") as "HΦ".
+      iModIntro; wp_pures. by iApply "HΦ".
+    + iDestruct "Hif" as "(Hl' & HR)"; iCombine "Hl Hl'" as "Hl".
+      rewrite Qp.quarter_three_quarter; wp_cmpxchg_suc.
+      rewrite -Qp.quarter_three_quarter; iDestruct "Hl" as "(Hl & Hl')".
+      iDestruct ("Hclose" $! true with "[Hl]") as ">AP".
+      { iExists l, true. by iFrame. }
+      iMod (atomic_post_commit with "AP") as "HΦ".
+      iModIntro; wp_pures. iApply "HΦ". 
+      iFrame "HR". iExists l. by iFrame.
+  Qed.
+
+  Lemma acquire_spec (lk: val) (R : iProp Σ) :
+    ⊢ <<< is_lock lk R >>> acquire lk @ ∅ 
+    <<< is_lock lk R, RET #() >>>
+    {{{ locked lk ∗ R }}}.
+  Proof.
+    iIntros (Φ) "AU"; rewrite difference_empty_L.
+    iLöb as "IH". wp_lam.
+    awp_apply try_acquire_spec.
+    iApply (aacc_aupd_eq with "AU"); try done.
+    iIntros "Hlock"; iAaccIntro with "Hlock".
+    { do 2 (iIntros; iModIntro; iFrame). }
+    iIntros ([]) "Hlock".
+    + iModIntro. iFrame "Hlock". iIntros "Hlock". 
+      iRight. iFrame. iIntros "AP".
+      iMod (atomic_post_commit with "AP") as "HΦ".
+      by iModIntro; iIntros; iModIntro; wp_pures; iApply "HΦ".
+    + iModIntro. iFrame "Hlock". iIntros "Hlock". 
+      iLeft. iFrame. iIntros "AP". 
+      by iModIntro; iIntros; iModIntro; wp_pures; iApply "IH".
+  Qed.
+
+  Lemma release_spec (lk: val) (R : iProp Σ) :
+    locked lk -∗ R -∗
+    <<< is_lock lk R >>> release lk @ ∅
+    <<< is_lock lk R, RET #() >>>
+    {{{ True }}}.
+  Proof.
+    iIntros "Hlocked HR" (Φ) "AU"; rewrite difference_empty_L.
+    wp_lam. iMod "AU" as "[Hlock [_ Hclose]]".
+    iDestruct "Hlock" as (l b) "(-> & Hl & _)".
+    iDestruct "Hlocked" as (l') "(%Heq & Hl')". 
+    symmetry in Heq; inversion Heq; subst.
+    iDestruct (mapsto_agree with "Hl Hl'") as %<-.
+    iCombine "Hl Hl'" as "Hl"; rewrite Qp.quarter_three_quarter.
+    wp_store. iMod ("Hclose" with "[Hl HR]") as "AP".
+    {
+      rewrite -Qp.quarter_three_quarter; iDestruct "Hl" as "(HlL & HlR)".
+      iExists l, false; by iFrame.
+    }
+    iMod "AP" as "[Hlock [_ HΦ]]". 
+    iMod ("HΦ" with "Hlock") as "HΦ".
+    by iApply "HΦ".
+  Qed.
+End proof.
