atomic/weakestpre.v
@@ -1,0 +1,221 @@
+From stdpp Require Import namespaces.
+From iris.bi Require Import telescopes.
+From iris.proofmode Require Import proofmode classes.
+From iris.program_logic Require Export weakestpre.
+From iris.base_logic Require Import invariants.
+From iris.prelude Require Import options.
+
+From SkipList.atomic Require Export update.
+
+(* This hard-codes the inner mask to be empty, because we have yet to find an
+example where we want it to be anything else. *)
+Definition atomic_wp `{!irisGS_gen hlc Λ Σ} {TA TB TC : tele}
+  (e: expr Λ) (* expression *)
+  (E : coPset) (* *implementation* mask *)
+  (α: TA → iProp Σ) (* atomic pre-condition *)
+  (β: TA → TB → iProp Σ) (* atomic post-condition *)
+  (Q: TA → TB → iProp Σ) (* private post-condition *)
+  (Ψ: TC → iProp Σ)
+  (f: TA → TB → val Λ) (* Turn the return data into the return value *)
+  : iProp Σ :=
+    ∀ (Φ : val Λ → iProp Σ),
+            (* The (outer) user mask is what is left after the implementation
+            opened its things. *)
+            atomic_update (⊤∖E) ∅ α Ψ β (λ.. x y, Q x y ={⊤∖E}=∗ Φ (f x y)) -∗
+            WP e {{ Φ }}.
+(* Note: To add a private postcondition, use
+   atomic_update α β Eo Ei (λ x y, POST x y -∗ Φ (f x y)) *)
+
+(* The way to read the [tele_app foo] here is that they convert the n-ary
+function [foo] into a unary function taking a telescope as the argument. *)
+Notation "'<<<' ∀∀ x1 .. xn , α '>>>' e @ E '<<<' ∃∃ y1 .. yn , β , 'RET' v '>>>' {{{ Q } } }" :=
+  (atomic_wp (TA:=TeleS (λ x1, .. (TeleS (λ xn, TeleO)) .. ))
+             (TB:=TeleS (λ y1, .. (TeleS (λ yn, TeleO)) .. ))
+             (TC:=TeleS (λ x1, .. (TeleS (λ xn, TeleO)) .. ))
+             e%E
+             E
+             (tele_app $ λ x1, .. (λ xn, α%I) ..)
+             (tele_app $ λ x1, .. (λ xn,
+                         tele_app (λ y1, .. (λ yn, β%I) .. )
+                        ) .. )
+             (tele_app $ λ x1, .. (λ xn,
+                         tele_app (λ y1, .. (λ yn, Q%I) .. )
+                        ) .. )
+             (tele_app $ λ x1, .. (λ xn, α%I) ..)
+             (tele_app $ λ x1, .. (λ xn,
+                         tele_app (λ y1, .. (λ yn, v%V) .. )
+                        ) .. )
+  )
+  (at level 20, E, α, β, Q, v at level 200, x1 binder, xn binder, y1 binder, yn binder,
+   format "'[hv' '<<<'  '[' ∀∀  x1  ..  xn ,  '/' α  ']' '>>>'  '/  ' e  @  E  '/' '<<<'  '[' ∃∃  y1  ..  yn ,  '/' β ,  '/' 'RET'  v  ']' '>>>' {{{ '[' Q ']' } } } ']'")
+  : bi_scope.
+
+Notation "'<<<' ∀∀ x1 .. xn , α '>>>' e @ E '<<<' β , 'RET' v '>>>' {{{ Q } } }" :=
+  (atomic_wp (TA:=TeleS (λ x1, .. (TeleS (λ xn, TeleO)) .. ))
+             (TB:=TeleO)
+             (TC:=TeleS (λ x1, .. (TeleS (λ xn, TeleO)) .. ))
+             e%E
+             E
+             (tele_app $ λ x1, .. (λ xn, α%I) ..)
+             (tele_app $ λ x1, .. (λ xn, tele_app β%I) .. )
+             (tele_app $ λ x1, .. (λ xn, tele_app Q%I) .. )
+             (tele_app $ λ x1, .. (λ xn, α%I) ..)
+             (tele_app $ λ x1, .. (λ xn, tele_app v%V) .. )
+  )
+  (at level 20, E, α, β, Q, v at level 200, x1 binder, xn binder,
+   format "'[hv' '<<<'  '[' ∀∀  x1  ..  xn ,  '/' α  ']' '>>>'  '/  ' e  @  E  '/' '<<<'  '[' β ,  '/' 'RET'  v  ']' '>>>' {{{ '[' Q ']' } } } ']'")
+  : bi_scope.
+
+Notation "'<<<' α '>>>' e @ E '<<<' ∃∃ y1 .. yn , β , 'RET' v '>>>' {{{ Q } } }" :=
+  (atomic_wp (TA:=TeleO)
+             (TB:=TeleS (λ y1, .. (TeleS (λ yn, TeleO)) .. ))
+             (TC:=TeleO)
+             e%E
+             E
+             (tele_app α%I)
+             (tele_app $ tele_app (λ y1, .. (λ yn, β%I) .. ))
+             (tele_app $ tele_app (λ y1, .. (λ yn, Q%I) .. ))
+             (tele_app α%I)
+             (tele_app $ tele_app (λ y1, .. (λ yn, v%V) .. ))
+  )
+  (at level 20, E, α, β, Q, v at level 200, y1 binder, yn binder,
+   format "'[hv' '<<<'  '[' α  ']' '>>>'  '/  ' e  @  E  '/' '<<<'  '[' ∃∃  y1  ..  yn ,  '/' β ,  '/' 'RET'  v  ']' '>>>' {{{ '[' Q ']' } } } ']'")
+  : bi_scope.
+
+Notation "'<<<' α '>>>' e @ E '<<<' β , 'RET' v '>>>' {{{ Q } } }" :=
+  (atomic_wp (TA:=TeleO)
+             (TB:=TeleO)
+             (TC:=TeleO)
+             e%E
+             E
+             (tele_app α%I)
+             (tele_app $ tele_app β%I)
+             (tele_app $ tele_app Q%I)
+             (tele_app α%I)
+             (tele_app $ tele_app v%V)
+  )
+  (at level 20, E, α, β, Q, v at level 200,
+   format "'[hv' '<<<'  '[' α  ']' '>>>'  '/  ' e  @  E  '/' '<<<'  '[' β ,  '/' 'RET'  v  ']' '>>>' {{{ '[' Q ']' } } } ']'")
+  : bi_scope.
+
+(** Theory *)
+Section lemmas.
+  Context `{!irisGS_gen hlc Λ Σ} {TA TB TC : tele}.
+  Notation iProp := (iProp Σ).
+  Implicit Types (α : TA → iProp) (β Q : TA → TB → iProp) (Ψ : TC → iProp) (f : TA → TB → val Λ).
+
+  (* Atomic triples imply sequential triples. *)
+  Lemma atomic_wp_seq e E α β Q Ψ f :
+    atomic_wp e E α β Q Ψ f -∗
+    ∀ Φ, ∀.. x, α x -∗
+    (∀.. y, β x y -∗ (Q x y -∗ Φ (f x y))) -∗
+    (∀.. y, β x y -∗ ∃.. z, Ψ z ∗ (Ψ z -∗ β x y)) -∗
+    WP e {{ Φ }}.
+  Proof.
+    iIntros "Hwp" (Φ x) "Hα HΦ HΨ".
+    iApply (wp_frame_wand with "HΦ"). iApply "Hwp".
+    iAuIntro. iAaccIntro with "Hα". 
+    { iIntros; iModIntro; iFrame. }
+    iIntros (y) "Hβ !>".
+    iDestruct ("HΨ" with "Hβ") as (z) "[HΨ Hβ]".
+    iExists z. iFrame "HΨ". iIntros "HΨ".
+    rewrite ->!tele_app_bind. iIntros "HQ !> HΦ".
+    iDestruct ("Hβ" with "HΨ") as "Hβ".
+    iApply ("HΦ" with "Hβ HQ").
+  Qed.
+
+  (** This version matches the Texan triple, i.e., with a later in front of the
+  [(∀.. y, β x y -∗ Φ (f x y))]. *)
+  Lemma atomic_wp_seq_step e E α β Q Ψ f :
+    TCEq (to_val e) None →
+    atomic_wp e E α β Q Ψ f -∗
+    ∀ Φ, ∀.. x, α x -∗
+    ▷ (∀.. y, β x y -∗ (Q x y -∗ Φ (f x y))) -∗
+    (∀.. y, β x y -∗ ∃.. z, Ψ z ∗ (Ψ z -∗ β x y)) -∗
+    WP e {{ Φ }}.
+  Proof.
+    iIntros (?) "H"; iIntros (Φ x) "Hα HΦ HΨ".
+    iApply (wp_step_fupd _ _ ⊤ _ (∀.. y, β x y -∗ (Q x y -∗ Φ (f x y)))
+      with "[$HΦ //]"); first done.
+    iApply (atomic_wp_seq with "H Hα [] HΨ").
+    iIntros (y) "Hβ HQ HΦ". iModIntro.
+    iApply ("HΦ" with "Hβ HQ").
+  Qed.
+
+  (* Sequential triples with the empty mask for a physically atomic [e] are atomic. *)
+  Lemma atomic_seq_wp_atomic e E α β Q Ψ f `{!Atomic WeaklyAtomic e} :
+    (∀ Φ, ∀.. x, α x -∗ (∀.. y, β x y -∗ (Q x y -∗ Φ (f x y))) -∗ WP e @ ∅ {{ Φ }}) -∗
+    atomic_wp e E α β Q Ψ f.
+  Proof.
+    iIntros "Hwp" (Φ) "AU". iMod "AU" as (x) "[Hα [_ Hclose]]".
+    iApply ("Hwp" with "Hα"). iIntros (y) "Hβ HQ".
+    iMod ("Hclose" with "Hβ") as "AP". rewrite ->!tele_app_bind. 
+    iMod "AP" as (z) "[HΨ [_ HΦ]]". iMod ("HΦ" with "HΨ") as "HΦ".
+    iDestruct ("HΦ" with "HQ") as "HΦ".
+    iApply fupd_mask_mono; last by iFrame.
+    solve_ndisj.
+  Qed.
+
+  (** Sequential triples with a persistent precondition and no initial quantifier
+  are atomic. *)
+  Lemma persistent_seq_wp_atomic e E (α : [tele] → iProp) 
+        (β : [tele] → TB → iProp) (Q : [tele] → TB → iProp) Ψ
+        (f : [tele] → TB → val Λ) {HP : Persistent (α [tele_arg])} :
+    (∀ Φ, α [tele_arg] -∗ 
+      (∀.. y, β [tele_arg] y -∗ (Q [tele_arg] y -∗ Φ (f [tele_arg] y))) -∗ WP e {{ Φ }}
+    ) -∗
+    atomic_wp e E α β Q Ψ f.
+  Proof.
+    simpl in HP. iIntros "Hwp" (Φ) "HΦ". iApply fupd_wp.
+    iMod ("HΦ") as "[#Hα [Hclose _]]". iMod ("Hclose" with "Hα") as "HΦ".
+    iApply wp_fupd. iApply ("Hwp" with "Hα"). iIntros "!>" (y) "Hβ HQ".
+    iMod ("HΦ") as "[_ [_ Hclose]]". iMod ("Hclose" with "Hβ") as "HΦ".
+    rewrite ->!tele_app_bind. iMod "HΦ" as (z) "[HΨ [_ HΦ]]".
+    iMod ("HΦ" with "HΨ") as "HΦ". iDestruct ("HΦ" with "HQ") as "HΦ".
+    iApply fupd_mask_mono; last by iFrame.
+    solve_ndisj.
+  Qed.
+
+  Lemma atomic_wp_mask_weaken e E1 E2 α β Q Ψ f :
+    E1 ⊆ E2 → atomic_wp e E1 α β Q Ψ f -∗ atomic_wp e E2 α β Q Ψ f.
+  Proof.
+    iIntros (HE) "Hwp". iIntros (Φ) "AU". iApply "Hwp".
+    iApply (atomic_update_mask_weaken (⊤ ∖ E2)); first solve_ndisj.
+    iApply (atomic_update_wand with "[] AU").
+    iIntros (x y) "HΦ". rewrite ->!tele_app_bind.
+    iIntros "HQ". iDestruct ("HΦ" with "HQ") as "HΦ".
+    iApply fupd_mask_mono; last by iFrame.
+    solve_ndisj.
+  Qed.
+
+  (** We can open invariants around atomic triples.
+      (Just for demonstration purposes; we always use [iInv] in proofs.) *)
+  Lemma atomic_wp_inv e E α β Q Ψ f N I :
+    ↑N ⊆ E →
+    (∀.. x y, β x y -∗ ∃.. z, Ψ z ∗ (Ψ z -∗ β x y)) -∗
+    atomic_wp e (E ∖ ↑N) (λ.. x, ▷ I ∗ α x) (λ.. x y, ▷ I ∗ β x y) Q Ψ f -∗
+    inv N I -∗ atomic_wp e E α β Q Ψ f.
+  Proof.
+    intros ?. iIntros "HβΨ Hwp #Hinv" (Φ) "AU". iApply "Hwp". 
+    iAuIntro. iInv N as "HI".
+    iApply (aacc_aupd with "AU"); first solve_ndisj. iIntros (x) "Hα".
+    iAaccIntro with "[HI Hα]"; rewrite ->!tele_app_bind; first by iFrame.
+    - (* abort *)
+      iIntros "[HI $]". by eauto with iFrame.
+    - (* commit *)
+      iIntros (y). rewrite ->!tele_app_bind. iIntros "[HI Hβ]".
+      iModIntro. iDestruct ("HβΨ" with "Hβ") as (z) "[HΨ Hβ]".
+      iExists z. iFrame "HΨ". iIntros "HΨ".
+      iRight. iExists y. rewrite ->!tele_app_bind.
+      iDestruct ("Hβ" with "HΨ") as "Hβ"; clear z.
+      iFrame "Hβ". iIntros "AP". iModIntro.
+      iApply (apst_apst_eq with "AP"); try done.
+      iIntros "AP". iModIntro. iFrame "HI".
+      iApply (atomic_post_mask_weaken (⊤ ∖ (E ∖ ↑N) ∖ ↑N)); first solve_ndisj.
+      iApply (atomic_post_wand with "[] AP").
+      iIntros "HΦ HQ". iDestruct ("HΦ" with "HQ") as "HΦ".
+      iApply fupd_mask_mono; last by iFrame.
+      solve_ndisj.
+  Qed.
+
+End lemmas.
