jelly_fish/rw_client/example.v
@@ -1,0 +1,115 @@
+From SkipList.atomic Require Import proofmode weakestpre.
+From SkipList.lib Require Import arg_max.
+From SkipList.jelly_fish Require Import code.
+From SkipList.jelly_fish.rw_client Require Import spec.
+
+From iris.heap_lang Require Import par notation.
+
+
+Module Params <: SKIP_LIST_PARAMS.
+  Local Open Scope Z.
+  Definition INT_MIN := -1000.
+  Definition INT_MAX := 1000.
+  Definition MAX_HEIGHT := 20.  
+  Lemma HMIN_MAX : INT_MIN < INT_MAX.
+  Proof. unfold INT_MIN, INT_MAX; lia. Qed.
+  Lemma HMAX_HEIGHT : 0 ≤ MAX_HEIGHT.
+  Proof. unfold MAX_HEIGHT; lia. Qed.
+End Params.
+
+Module Import Spec := RWSpec Params.
+
+Definition exampleN := nroot .@ "example".
+
+Definition skip_list_client : expr := 
+  let: "p" := new #() in
+    ((put "p" #10 #1 #0;; put "p" #20 #5 #1;; put "p" #10 #3 #2)
+    |||
+    (put "p" #20 #2 #0;; put "p" #10 #6 #1;; put "p" #10 #4 #2));;
+    (get "p" #10 ||| get "p" #20).
+
+Section Proofs.
+  Context `{!heapGS Σ, !rwG Σ, !spawnG Σ}.
+  Local Open Scope Z.
+
+  Lemma skip_list_client_spec :
+    {{{ True }}}
+      skip_list_client
+    {{{ (v: Z), RET (SOMEV (#v, #2), SOMEV (#5, #1)); ⌜ v = 3 ∨ v = 4 ⌝ }}}.
+  Proof.
+    iIntros (Φ) "_ HΦ".
+
+    unfold skip_list_client.
+    wp_apply new_spec; first done.
+    iIntros (p mΓ) "Hmap".
+    iDestruct (rw_inv_alloc_mut exampleN with "Hmap") as ">Hinv".
+    iDestruct "Hinv" as (Γ) "[#Hinv Hmut]".
+
+    wp_let.
+    rewrite -(Qp.div_2 1); iDestruct (mut_map_sep with "Hmut") as "[Hmut1 Hmut2]".
+    wp_smart_apply (wp_par (λ _, mut_map _ _ _) (λ _, mut_map _ _ _) with "[Hmut1] [Hmut2]").
+    {
+      awp_apply (write_spec with "Hinv"); first rewrite /Params.INT_MIN/Params.INT_MAX//.
+      iAaccIntro with "Hmut1"; first (iIntros "?"; iModIntro; iFrame).
+      iIntros "Hmut1". iModIntro. iExists _, _. iFrame "Hmut1".
+      iIntros "Hmut1 _". iModIntro. wp_pures.
+
+      awp_apply (write_spec with "Hinv"); first rewrite /Params.INT_MIN/Params.INT_MAX//.
+      iAaccIntro with "Hmut1"; first (iIntros "?"; iModIntro; iFrame).
+      iIntros "Hmut1". iModIntro. iExists _, _. iFrame "Hmut1".
+      iIntros "Hmut1 _". iModIntro. wp_pures.
+
+      awp_apply (write_spec with "Hinv"); first rewrite /Params.INT_MIN/Params.INT_MAX//.
+      iAaccIntro with "Hmut1"; first (iIntros "?"; iModIntro; iFrame).
+      iIntros "Hmut1". iModIntro. iExists _, _. iFrame "Hmut1".
+      by iIntros.
+    }
+    {
+      awp_apply (write_spec with "Hinv"); first rewrite /Params.INT_MIN/Params.INT_MAX//.
+      iAaccIntro with "Hmut2"; first (iIntros "?"; iModIntro; iFrame).
+      iIntros "Hmut2". iModIntro. iExists _, _. iFrame "Hmut2".
+      iIntros "Hmut2 _". iModIntro. wp_pures.
+
+      awp_apply (write_spec with "Hinv"); first rewrite /Params.INT_MIN/Params.INT_MAX//.
+      iAaccIntro with "Hmut2"; first (iIntros "?"; iModIntro; iFrame).
+      iIntros "Hmut2". iModIntro. iExists _, _. iFrame "Hmut2".
+      iIntros "Hmut2 _". iModIntro. wp_pures.
+
+      awp_apply (write_spec with "Hinv"); first rewrite /Params.INT_MIN/Params.INT_MAX//.
+      iAaccIntro with "Hmut2"; first (iIntros "?"; iModIntro; iFrame).
+      iIntros "Hmut2". iModIntro. iExists _, _. iFrame "Hmut2".
+      by iIntros.
+    }
+    iIntros (? ?) "Hmut". rewrite ?left_id_L.
+    iDestruct (mut_map_join with "Hmut") as "Hmut".
+
+    iNext; wp_pure; wp_pure.
+    rewrite Qp.div_2; iDestruct (mut_to_const with "Hinv Hmut") as ">Hconst".
+    rewrite -(Qp.div_2 1); iDestruct (const_map_sep with "Hconst") as "[Hconst1 Hconst2]".
+    wp_smart_apply (wp_par 
+      (λ v, ⌜ v = SOMEV (#3, #2) ∨ v = SOMEV (#4, #2) ⌝%I) 
+      (λ v, ⌜ v = SOMEV (#5, #1) ⌝%I)
+    with "[Hconst1] [Hconst2]").
+    {
+      awp_apply (read_spec with "Hinv"); first rewrite /Params.INT_MIN/Params.INT_MAX//.
+      iAaccIntro with "Hconst1"; first (iIntros "?"; iModIntro; iFrame).
+      iIntros (opt) "[Hconst1 %Hopt]". iModIntro. iExists _, _. iFrame "Hconst1".
+      iIntros "_ _"; iPureIntro.
+      destruct Hopt as (vs & v & t & Hprod & Hin & Hopt).
+      rewrite arg_max_eq in Hprod; inversion Hprod; subst.
+      rewrite elem_of_union ?elem_of_singleton in Hin.
+      destruct Hin; subst; first (by left); last (by right).
+    }
+    {
+      awp_apply (read_spec with "Hinv"); first rewrite /Params.INT_MIN/Params.INT_MAX//.
+      iAaccIntro with "Hconst2"; first (iIntros "?"; iModIntro; iFrame).
+      iIntros (opt) "[Hconst2 %Hopt]". iModIntro. iExists _, _. iFrame "Hconst2".
+      iIntros "_ _"; iPureIntro.
+      destruct Hopt as (vs & v & t & Hprod & Hin & Hopt).
+      rewrite comm_L arg_max_lt // in Hprod; inversion Hprod; subst.
+      rewrite elem_of_singleton in Hin; by subst.
+    }
+    iIntros (? ?) "[[->|->] ->]"; iNext; iApply "HΦ"; 
+      first (by iLeft); last (by iRight).
+  Qed.
+End Proofs.
