jelly_fish/rw_client/spec.v
@@ -1,0 +1,245 @@
+From SkipList.lib Require Import arg_max gmap_extra.
+From SkipList.atomic Require Import proofmode weakestpre.
+From SkipList.jelly_fish Require Import code inv.
+From SkipList.jelly_fish.spec Require Import new get put.
+
+From iris.algebra Require Import frac_auth gmap.
+From iris.base_logic.lib Require Import invariants.
+From iris.heap_lang Require Import notation.
+
+
+Class rwG Σ := RWG { 
+  rw_mutG :> inG Σ (frac_authR (gmapR Z (argmax Z)));
+  rw_agrG :> inG Σ (frac_authR (agreeR (gmap Z (argmax Z))));
+  rw_setG :> skipG Σ
+}.
+
+Record rw_gname := mk_rw_gname {
+  mut_gname: gname;
+  agr_gname: gname
+}.
+
+Module RWSpec (Params: SKIP_LIST_PARAMS).
+  Import Params.
+  Module New := NewSpec Params.
+  Module Get := GetSpec Params.
+  Module Put := PutSpec Params.
+  Export New Get Put.
+
+  Section invariant.
+    Context `{!heapGS Σ, !rwG Σ} (N: namespace).
+
+    Definition rw_mapN := N .@ "rw_map".
+
+    (* Public state for concurrent writes *)
+    Definition mut_map (m: gmap Z (argmax Z)) (q: frac) (Γ: rw_gname) : iProp Σ := 
+      own Γ.(mut_gname) (◯F{q} m).
+    Lemma mut_map_sep (m: gmap Z (argmax Z)) (q1 q2: frac) (Γ: rw_gname) :
+      mut_map m (q1 + q2) Γ -∗ mut_map m q1 Γ ∗ mut_map m q2 Γ.
+    Proof. iIntros "(Hmut1 & Hmut2)"; iFrame. Qed.
+    Lemma mut_map_join (m1 m2: gmap Z (argmax Z)) (q1 q2: frac) (Γ: rw_gname) :
+      mut_map m1 q1 Γ ∗ mut_map m2 q2 Γ -∗ mut_map (m1 ⋅ m2) (q1 + q2) Γ.
+    Proof. iIntros "(Hmut1 & Hmut2)"; by iCombine "Hmut1 Hmut2" as "Hmut". Qed.
+
+    (* Public state for concurrent reads *)
+    Definition const_map (m: gmap Z (argmax Z)) (q: frac) (Γ: rw_gname) : iProp Σ := 
+      own Γ.(agr_gname) (◯F{q} (to_agree m)).
+    Lemma const_map_sep (m: gmap Z (argmax Z)) (q1 q2: frac) (Γ: rw_gname) :
+      const_map m (q1 + q2) Γ -∗ const_map m q1 Γ ∗ const_map m q2 Γ.
+    Proof. iIntros "(Hmut1 & Hmut2)"; iFrame. Qed.
+    Lemma const_map_join (m: gmap Z (argmax Z)) (q1 q2: frac) (Γ: rw_gname) :
+      const_map m q1 Γ ∗ const_map m q2 Γ -∗ const_map m (q1 + q2) Γ.
+    Proof. iIntros "(Hmut1 & Hmut2)"; by iCombine "Hmut1 Hmut2" as "Hmut". Qed.
+
+    (* Definitions to construct the abstract map from the physical map*)
+    Fixpoint vs_to_set (vl: list tval) (t: Z) : gset Z :=
+      match vl with
+      | nil => ∅
+      | vt :: vl => if (decide (Z.lt vt.2 t)) then ∅
+                   else {[vt.1]} ∪ vs_to_set vl t
+      end.
+    Definition f_vs (vt: tval * list tval) : argmax Z := 
+      prodZ ({[vt.1.1]} ∪ vs_to_set vt.2 vt.1.2) vt.1.2.
+
+    (* Invariant concealing the abstract state of the full map *)
+    Definition map_inv (p: loc) (mΓ: gmap Z lazy_gname) (Γ: rw_gname) : iProp Σ :=
+      ∃ (m: gmap Z (tval * list tval)),
+        vc_map p m mΓ
+        ∗
+        own Γ.(mut_gname) (●F (f_vs <$> m : gmap Z (argmax Z)))
+        ∗
+        own Γ.(agr_gname) (●F (to_agree (f_vs <$> m : gmap Z (argmax Z))))
+        ∗
+        (own Γ.(mut_gname) (◯F (f_vs <$> m : gmap Z (argmax Z))) ∨ 
+        own Γ.(agr_gname) (◯F (to_agree (f_vs <$> m : gmap Z (argmax Z))))).
+    Definition is_map (p: loc) (Γ: rw_gname) : iProp Σ :=
+      ∃ (mΓ: gmap Z lazy_gname), inv rw_mapN (map_inv p mΓ Γ).
+    Lemma rw_inv_alloc_mut (p: loc) (mΓ: gmap Z lazy_gname) :
+      vc_map p ∅ mΓ ={⊤}=∗
+        ∃ (Γ: rw_gname), is_map p Γ ∗ mut_map ∅ 1 Γ.
+    Proof.
+      iIntros "Hmap".
+      iMod (own_alloc (●F ∅ ⋅ ◯F ∅))
+        as (γmut) "[Hmut● Hmut◯]"; first by apply auth_both_valid.
+      iMod (own_alloc (●F (to_agree ∅) ⋅ ◯F (to_agree ∅)))
+        as (γagr) "[Hagr● Hagr◯]"; first by apply auth_both_valid.
+      set (Γ := mk_rw_gname γmut γagr).
+      iMod (inv_alloc rw_mapN ⊤ (map_inv p mΓ Γ)
+        with "[Hmap Hmut● Hagr● Hagr◯]") as "#Hinv".
+      { iNext; iExists ∅; rewrite fmap_empty; iFrame. }
+      iModIntro; iExists Γ; iFrame "# ∗"; by iExists mΓ.
+    Qed.
+    Lemma rw_inv_alloc_const (p: loc) (mΓ: gmap Z lazy_gname) :
+      vc_map p ∅ mΓ ={⊤}=∗
+        ∃ (Γ: rw_gname), is_map p Γ ∗ const_map ∅ 1 Γ.
+    Proof.
+      iIntros "Hmap".
+      iMod (own_alloc (●F ∅ ⋅ ◯F ∅))
+        as (γmut) "[Hmut● Hmut◯]"; first by apply auth_both_valid.
+      iMod (own_alloc (●F (to_agree ∅) ⋅ ◯F (to_agree ∅)))
+        as (γagr) "[Hagr● Hagr◯]"; first by apply auth_both_valid.
+      set (Γ := mk_rw_gname γmut γagr).
+      iMod (inv_alloc rw_mapN ⊤ (map_inv p mΓ Γ)
+        with "[Hmap Hmut● Hagr● Hmut◯]") as "#Hinv".
+      { iNext; iExists ∅; rewrite fmap_empty; iFrame. }
+      iModIntro; iExists Γ; iFrame "# ∗"; by iExists mΓ.
+    Qed.
+
+    (* Helper lemmas for switching between concurrent writes and concurrent reads *)
+    Lemma mut_to_const (p: loc) (m: gmap Z (argmax Z)) (Γ: rw_gname) :
+      is_map p Γ -∗ mut_map m 1 Γ ={⊤}=∗ const_map m 1 Γ.
+    Proof.
+      rewrite /mut_map/const_map; iIntros "[%mΓ #Hinv] Hmut◯".
+      iInv "Hinv" as (m') ">(Hmap & Hmut● & Hagr● & Hagr◯)".
+      iDestruct (own_valid_2 with "Hmut● Hmut◯") as %<-%frac_auth_agree_L.
+      iDestruct "Hagr◯" as "[Hfalse|Hagr◯]".
+      { by iDestruct (own_valid_2 with "Hmut◯ Hfalse") as %[Hfalse%Qp.not_add_le_r _]%frac_auth_frag_valid. }
+      iModIntro. iSplitR "Hagr◯"; last (iModIntro; iFrame).
+      iNext; iExists m'; iFrame.
+    Qed.
+    Lemma const_to_mut (p: loc) (m: gmap Z (argmax Z)) (Γ: rw_gname) :
+      is_map p Γ -∗ const_map m 1 Γ ={⊤}=∗ mut_map m 1 Γ.
+    Proof.
+      rewrite /mut_map/const_map; iIntros "[%mΓ #Hinv] Hagr◯".
+      iInv "Hinv" as (m') ">(Hmap & Hmut● & Hagr● & Hmut◯)".
+      iDestruct (own_valid_2 with "Hagr● Hagr◯") as %Heq%frac_auth_agree.
+      replace m with (f_vs <$> m') by rewrite -to_agree_op_valid_L Heq agree_idemp //.
+      iDestruct "Hmut◯" as "[Hmut◯|Hfalse]"; last first.
+      { by iDestruct (own_valid_2 with "Hagr◯ Hfalse") as %[Hfalse%Qp.not_add_le_r _]%frac_auth_frag_valid. }
+      iModIntro. iSplitR "Hmut◯"; last (iModIntro; iFrame).
+      iNext; iExists m'; iFrame.
+    Qed.
+  End invariant.
+
+  Section proofs.
+    Context `{!heapGS Σ, !rwG Σ} (N: namespace).
+    Local Open Scope Z.
+
+    Definition opt_equiv (ret: val) (opt: option (argmax Z)) : iProp Σ :=
+      match opt with
+      | None => ⌜ ret = NONEV ⌝
+      | Some vt => ∃ (vs: gset Z) (v t: Z), 
+                     ⌜ vt = prodZ vs t ⌝ ∗ ⌜ v ∈ vs ⌝ ∗ ⌜ ret = SOMEV (#v, #t) ⌝
+      end.
+
+    Theorem read_spec (p: loc) (Γ: rw_gname)
+      (k: Z) (Hrange: INT_MIN < k < INT_MAX) :
+      is_map N p Γ -∗
+      <<< ∀∀ m q, const_map m q Γ >>>
+        get #p #k @ ↑N
+      <<< ∃∃ opt, const_map m q Γ ∗ opt_equiv opt (m !! k), RET opt >>>
+      {{{ True }}}.
+    Proof.
+      iIntros "[%mΓ #Hinv] %Φ AU".
+
+      awp_apply get_spec; first done.
+      iInv "Hinv" as (m) ">(Hmap & Hmut● & Hagr● & Hmut◯)".
+      iAaccIntro with "Hmap".
+      { iIntros; iModIntro; iFrame; iNext; iExists m; iFrame. }
+      iIntros "Hmap".
+
+      iMod "AU" as (m' q) "[Hagr◯ [_ Hclose]]".
+      iDestruct (own_valid_2 with "Hagr● Hagr◯") as %Heq%frac_auth_included.
+      rewrite Some_included_total to_agree_included leibniz_equiv_iff in Heq; subst.
+      iMod ("Hclose" $! (opt_to_val (m !! k)) with "[Hagr◯]") as "AP".
+      { 
+        iFrame "Hagr◯". rewrite lookup_fmap. 
+        destruct (m !! k) as [[[v t] vl]|]; last done.
+        simpl. iExists ({[v]} ∪ vs_to_set vl t), v, t.
+        iSplit; first done. iSplit; last done.
+        iPureIntro; set_solver.
+      }
+      iMod (atomic_post_commit with "AP") as "HΦ".
+
+      iModIntro. iExists m. iFrame "Hmap". iIntros "Hmap".
+      iSplitR "HΦ"; first (iNext; iExists m; iFrame).
+      iApply (apst_inv with "Hinv [HΦ]"); first solve_ndisj.
+      { iIntros. iApply fupd_mask_mono; last by iApply "HΦ". solve_ndisj. }
+      clear m; iIntros "!> [%m [Hmap ?]]". iExists m.
+      iFrame "Hmap". iIntros "Hmap". iExists m. iFrame.
+    Qed.
+
+    Theorem write_spec (p: loc) (Γ: rw_gname)
+      (k v t: Z) (Hrange: INT_MIN < k < INT_MAX) :
+      is_map N p Γ -∗
+      <<< ∀∀ m q, mut_map m q Γ >>>
+        put #p #k #v #t @ ↑N
+      <<< mut_map (m ⋅ {[ k := prodZ {[v]} t]}) q Γ, RET #() >>>
+      {{{ True }}}.
+    Proof.
+      iIntros "[%mΓ #Hinv] %Φ AU".
+
+      awp_apply put_spec; first done.
+      iInv "Hinv" as (m) ">(Hmap & Hmut● & Hagr● & Hagr◯)".
+      iAaccIntro with "Hmap".
+      { iIntros; iModIntro; iFrame; iNext; iExists m; iFrame. }
+      iIntros "Hmap".
+
+      iMod "AU" as (m' q) "[Hmut◯ [_ Hclose]]".
+      iMod (own_update_2 with "Hmut● Hmut◯") as "[Hmut● Hmut◯]".
+      { 
+        apply frac_auth_update, (op_local_update_discrete _ _ {[ k := prodZ {[v]} t]}). 
+        destruct ((f_vs <$> m) !! k) eqn:Hopt.
+        + rewrite -(insert_singleton_op_Some_L _ _ _ _ Hopt).
+          by apply insert_valid.
+        + rewrite -(insert_singleton_op _ _ _ Hopt).
+          by apply insert_valid.
+      }
+      do 2 rewrite (comm _ {[k := prodZ {[v]} t]} _).
+      iDestruct "Hagr◯" as "[Hfalse|Hagr◯]".
+      { by iDestruct (own_valid_2 with "Hmut◯ Hfalse") as %[Hfalse%Qp.not_add_le_r _]%frac_auth_frag_valid. }
+      iMod (own_update_2 with "Hagr● Hagr◯") as "[Hagr● Hagr◯]".
+      { by apply (frac_auth_update_1 _ _ (to_agree ((f_vs <$> m) ⋅ {[k := prodZ {[v]} t]}))). }
+      iMod ("Hclose" with "[$]") as "AP".
+      iMod (atomic_post_commit with "AP") as "HΦ".
+
+      iModIntro. iExists (case_map m k v t). iFrame "Hmap". iIntros "Hmap".
+      assert ((f_vs <$> m) ⋅ {[k := prodZ {[v]} t]} = f_vs <$> case_map m k v t) as Heq.
+      { 
+        destruct ((f_vs <$> m) !! k) eqn:Hopt.
+        + rewrite comm_L -(insert_singleton_op_Some_L _ _ _ _ Hopt).
+          rewrite lookup_fmap fmap_Some in Hopt; destruct Hopt as [[vt vl] [Hopt Hf]].
+          rewrite /case_map Hopt Hf.
+          case_decide.
+          - rewrite insert_id // lookup_fmap Hopt fmap_Some.
+            exists (vt, vl). split; first done.
+            rewrite /f_vs arg_max_lt //.
+          - rewrite fmap_insert {1 3}/f_vs /=.
+            case_decide.
+            * rewrite right_id_L comm_L arg_max_lt //. 
+            * replace t with vt.2 by lia.
+              rewrite arg_max_eq //.
+        + rewrite comm_L -(insert_singleton_op _ _ _ Hopt).
+          rewrite lookup_fmap fmap_None in Hopt.
+          rewrite /case_map Hopt fmap_insert.
+          rewrite {2}/f_vs //= right_id_L //.
+      }
+      rewrite Heq.
+      iSplitR "HΦ"; first (iNext; iExists (case_map m k v t); iFrame).
+      iApply (apst_inv with "Hinv [HΦ]"); first solve_ndisj.
+      { iIntros. iApply fupd_mask_mono; last by iApply "HΦ". solve_ndisj. }
+      clear dependent m; iIntros "!> [%m [Hmap ?]]". iExists m.
+      iFrame "Hmap". iIntros "Hmap". iExists m. iFrame.
+    Qed.
+  End proofs.
+End RWSpec.
