jelly_fish/spec/find.v
@@ -1,9 +1,7 @@
-From iris.algebra Require Import gmap gset excl_auth dfrac_agree.
-From iris.base_logic.lib Require Import invariants.
-From iris.program_logic Require Import atomic.
-From iris.heap_lang Require Import proofmode.
+From iris.heap_lang Require Import notation.
 
 From SkipList.lib Require Import zrange.
+From SkipList.atomic Require Import weakestpre proofmode lock.
 From SkipList.jelly_fish Require Import code inv.
 
 
@@ -13,192 +11,161 @@ Module FindSpec (Params: SKIP_LIST_PARAMS).
   Export Invariant.
 
   Section proofs.
-    Context `{!heapGS Σ, !skipG Σ} (N: namespace).
+    Context `{!heapGS Σ, !skipG Σ}.
     Local Open Scope Z.
-    
-    Theorem find_spec (k lvl: Z) (head curr: node_rep) (Γm: map_gname) (Γ: gmap Z inv_gname) :
+
+    Theorem find_spec (k: Z) (head curr: node_rep) (Γ: lazy_gname)
+      (γ: option lazy_gname) (lvl: Z) :
       node_key curr < k < INT_MAX →
-      0 ≤ lvl ≤ MAX_HEIGHT →
-      (⌜ curr = head ⌝ ∨ own (Γ !!! lvl).(auth_gname) (◯ {[curr]})) -∗
-      inv (skipN N) (skip_list_inv head Γm Γ) -∗
-      <<< ∀∀ (s: gset Z), own Γm.(excl_gname) (◯E s) >>>
-        find (rep_to_node curr) #k #lvl @ ↑(skipN N)
-      <<< ∃∃ pred succ,
-        own Γm.(excl_gname) (◯E s)
+      (⌜ curr = head ⌝ ∨ own Γ.(auth_gname) (◯ {[curr]})) -∗
+      <<< ∀∀ S, lazy_list head S Γ γ lvl >>>
+        find (rep_to_node curr) #k #lvl @ ∅
+      <<< ∃∃ pred succ, 
+        lazy_list head S Γ γ lvl
         ∗
-        ⌜ k ≠ node_key succ → lvl = 0 → k ∉ s ⌝
+        ⌜ k ≠ node_key succ → k ∉ (set_map node_key S : gset Z) ⌝, 
+      RET ((rep_to_node pred), (rep_to_node succ)) >>>
+      {{{ 
+        (⌜ pred = head ⌝ ∨ own Γ.(auth_gname) (◯ {[pred]}))
         ∗
-        (⌜ pred = head ⌝ ∨ own (Γ !!! lvl).(auth_gname) (◯ {[pred]}))
-        ∗
-        (⌜ succ = tail ⌝ ∨ own (Γ !!! lvl).(auth_gname) (◯ {[succ]}))
+        (⌜ succ = tail ⌝ ∨ own Γ.(auth_gname) (◯ {[succ]}))
         ∗
         ⌜ node_key pred < k ≤ node_key succ ⌝
-        ∗
-        has_lock lvl pred,
-      RET ((rep_to_node pred), (rep_to_node succ)) >>>.
+      }}}.
     Proof.
-      iIntros "%Hk %Hlvl Hcurr #Hinv %Φ"; iRevert (curr Hk) "Hcurr".
-      iLöb as "IH"; iIntros "%curr %Hk #Hcurr AU".
+      iIntros "%Hk Hcurr %Φ"; iRevert (curr Hk) "Hcurr".
+      iLöb as "IH"; iIntros (curr Hk) "#Hcurr AU".
+      rewrite difference_empty_L.
       wp_lam. wp_let. wp_let. wp_lam. wp_pures.
 
-      wp_bind (Load #(node_next curr +ₗ lvl)). iInv "Hinv" as "Hskip". 
-      iDestruct (has_lvl_inv with "Hskip") as "(Hlvl & Hskip)"; first done.
-      iDestruct "Hlvl" as (S) "(>Hauth & >Hdisj & >Htoks & Hlocks & Hnexts & Hmap)".
-
-      iDestruct (singleton_frag_in with "Hauth Hcurr") as %Hcurr.
-      rewrite (big_sepS_delete (has_lock _)) // (big_sepS_delete (has_next _ _)) //.
-      iDestruct "Hlocks" as "(#Hlock & Hlocks)"; iDestruct "Hnexts" as "(Hnext & Hnexts)".
-      iDestruct "Hnext" as (s succ) ">(Hnext & #Hs & #Hsucc & Hkeys)".
-
+      wp_bind (Load #(_)). iMod "AU" as (S) "[Hlazy Hclose]".
+      iDestruct (singleton_frag_in with "Hcurr Hlazy") as %Hcurr.
+      iDestruct (node_has_next with "Hcurr Hlazy")
+        as (s succ) "(Hnext & #Hs & #Hsucc & %Hdisj & Hlazy)".
       destruct (decide (k ≤ node_key succ)) as [|Hcase].
-      + iMod "AU" as (d) "[Hexcl◯ [_ Hclose]]".
-        iDestruct (own_valid_2 with "Hdisj Hkeys") as %[Hdisj _]%ZRange_disj.
-        iDestruct (singleton_frag_in with "Hauth Hsucc") as %Hsucc%elem_of_union.
-        rewrite elem_of_singleton in Hsucc.
-
-        wp_load.
-        iAssert (has_next _ _ curr) with "[Hnext Hkeys]" as "Hnext".
-        { iExists s, succ; iFrame "# ∗". }
-        iCombine "Hlock Hlocks" as "Hlocks"; iCombine "Hnext Hnexts" as "Hnexts".
-        do 2 rewrite -big_sepS_delete //.
-
-        iAssert ⌜ lvl = 0 → set_map node_key S = d ⌝%I with "[Hmap Hexcl◯]" as %Heqd.
-        { 
-          iIntros (->); iDestruct "Hmap" as "(Hexcl● & _)".
-          by iDestruct (own_valid_2 with "Hexcl● Hexcl◯") as %<-%excl_auth_agree_L.
-        }
-        iDestruct ("Hclose" with "[Hexcl◯]") as ">HΦ"; last iModIntro.
+      + wp_load. iDestruct ("Hlazy" with "Hnext") as "Hlazy".
+        iDestruct "Hclose" as "[_ Hclose]".
+        iDestruct ("Hclose" $! curr succ with "[-]") as ">AP".
         {
-          iFrame "# ∗"; iPureIntro; split; last lia.
-          intros Hneq <-%Heqd Hfalse.
-          by apply (Hdisj k); last (rewrite zrange_spec; lia).
+          iDestruct (singleton_frag_in with "Hsucc Hlazy") as %Hsucc.
+          rewrite elem_of_union elem_of_singleton in Hsucc.
+          iFrame "Hlazy"; iPureIntro. intros Hneq Hin%Hdisj. 
+          apply Hin. rewrite zrange_spec; lia.
         }
-
-        iModIntro; iSplitR "HΦ".
-        { iNext; iApply "Hskip"; iExists S; iFrame. }
-        wp_load; wp_let; wp_lam; wp_pures.
+        iMod (atomic_post_commit with "AP") as "HΦ".
+        iModIntro. wp_load; wp_let; wp_lam; wp_pures.
         case_bool_decide; last lia; wp_if.
-        by wp_pure.
-      + wp_load.
-        iAssert (has_next _ _ curr) with "[Hnext Hkeys]" as "Hnext".
-        { iExists s, succ; iFrame "# ∗". }
-        iCombine "Hlock Hlocks" as "Hlocks"; iCombine "Hnext Hnexts" as "Hnexts".
-        do 2 rewrite -big_sepS_delete //.
-
-        iModIntro; iSplitR "AU".
-        { iNext; iApply "Hskip"; iExists S; iFrame. }
-        wp_load; wp_let; wp_lam; wp_pures.
+        wp_pure. iApply "HΦ".
+        iFrame "#". iPureIntro; lia.
+      + wp_load. iDestruct ("Hlazy" with "Hnext") as "Hlazy".
+        iDestruct "Hclose" as "[Hclose _]".
+        iDestruct ("Hclose" with "Hlazy") as ">AU".
+        iModIntro; wp_load; wp_let; wp_lam; wp_pures.
         case_bool_decide; first lia; wp_if.
+
         iDestruct "Hsucc" as "[->|Hsucc]"; first (rewrite /node_key/= in Hcase; lia).
         iApply ("IH" with "[%] [$] AU"); lia.
     Qed.
 
-    Theorem findLock_spec (k lvl: Z) (head curr: node_rep) (Γm: map_gname) (Γ: gmap Z inv_gname) :
+    Theorem findLock_spec (k: Z) (head curr: node_rep) (Γ: lazy_gname)
+      (γ: option lazy_gname) (lvl: Z) :
       node_key curr < k < INT_MAX →
-      0 ≤ lvl ≤ MAX_HEIGHT →
-      (⌜ curr = head ⌝ ∨ own (Γ !!! lvl).(auth_gname) (◯ {[curr]})) -∗
-      inv (skipN N) (skip_list_inv head Γm Γ) -∗
-      <<< ∀∀ (s: gset Z), own Γm.(excl_gname) (◯E s) >>>
-        findLock (rep_to_node curr) #k #lvl @ ↑(skipN N)
+      (⌜ curr = head ⌝ ∨ own Γ.(auth_gname) (◯ {[curr]})) -∗
+      <<< ∀∀ S, lazy_list head S Γ γ lvl >>>
+        findLock (rep_to_node curr) #k #lvl @ ∅
       <<< ∃∃ pred succ,
-        own Γm.(excl_gname) (◯E s)
+        lazy_list head S Γ γ lvl
         ∗
-        ⌜ k ≠ node_key succ → lvl = 0 → k ∉ s ⌝
+        ⌜ k ≠ node_key succ → k ∉ (set_map node_key S : gset Z) ⌝,
+      RET ((rep_to_node pred), (rep_to_node succ)) >>>
+      {{{
+        (⌜ pred = head ⌝ ∨ own Γ.(auth_gname) (◯ {[pred]}))
         ∗
-        (⌜ pred = head ⌝ ∨ own (Γ !!! lvl).(auth_gname) (◯ {[pred]}))
-        ∗
-        (⌜ succ = tail ⌝ ∨ own (Γ !!! lvl).(auth_gname) (◯ {[succ]}))
+        (⌜ succ = tail ⌝ ∨ own Γ.(auth_gname) (◯ {[succ]}))
         ∗
         ⌜ node_key pred < k ≤ node_key succ ⌝
         ∗
-        ∃ (γl: gname) (l: val) (s: loc), 
-          (node_lock pred +ₗ lvl) ↦□ l
-          ∗
-          is_lock γl l (in_lock lvl (node_next pred))
-          ∗
+        ∃ (s: loc),
           (node_next pred +ₗ lvl) ↦{#1 / 2} #s
           ∗
           s ↦□ rep_to_node succ
           ∗
           locked_val lvl s
           ∗
-          locked γl,
-      RET ((rep_to_node pred), (rep_to_node succ)) >>>.
+          locked #(node_lock pred +ₗ lvl)
+      }}}.
     Proof.
-      iIntros "%Hk %Hlvl Hcurr #Hinv %Φ"; iRevert (curr Hk) "Hcurr".
+      iIntros "%Hk Hcurr %Φ"; iRevert (curr Hk) "Hcurr".
       iLöb as "IH"; iIntros (curr Hk) "#Hcurr AU".
+      rewrite difference_empty_L.
       wp_lam. wp_let. wp_let.
-      
-      awp_apply (find_spec with "Hcurr Hinv"); first done; first done.
-      iApply (aacc_aupd with "AU"); first done.
-      iIntros (d) "Hexcl◯"; iAaccIntro with "Hexcl◯".
-      { do 2 (iIntros "?"; iModIntro; iFrame). }
-      iIntros (pred succ') "(Hexcl◯ & _ & #Hpred & _ & (%Hk' & _) & Hlock)".
-      iDestruct "Hlock" as (γl l) "(#Hlock & #His_lock)".
 
-      iModIntro; iLeft; iFrame. 
-      iIntros "AU"; iModIntro.
-      wp_pures; wp_lam; wp_pures; wp_load; wp_let.
+      awp_apply (find_spec with "Hcurr"); first done.
+      iApply (aacc_aupd_eq with "AU"); try done.
+      iIntros (S) "Hlazy"; iAaccIntro with "Hlazy".
+      { do 2 (iIntros; iModIntro; iFrame). }
+      iIntros (pred succ') "[Hlazy _]".
+      iModIntro. iExists S. iFrame "Hlazy". iIntros "Hlazy".
+      iLeft. iFrame "Hlazy". clear dependent S. iIntros "AU".
+      iModIntro. iIntros "(#Hpred & _ & [%Hk' _])".
+      iModIntro. wp_pures; wp_lam; wp_pures.
 
-      wp_bind (acquire _).
-      iApply (acquire_spec with "His_lock").
-      iNext; iIntros "(Hlocked & Hin_lock)".
-      iDestruct "Hin_lock" as (s) "(Hnext' & Hval)".
-      wp_pures; wp_lam; wp_pures.
+      awp_apply acquire_spec.
+      iApply (aacc_aupd_sub with "[] AU"); try done.
+      { iIntros "!> %S H"; iDestruct (node_has_lock with "Hpred H") as "$". }
+      iIntros (S) "Hlazy".
+      iDestruct (node_has_lock with "Hpred Hlazy") as "[Hlock Hlazy]".
+      iAaccIntro with "Hlock".
+      { iIntros "H"; iDestruct ("Hlazy" with "H") as "Hlazy"; iModIntro; iFrame; by iIntros. }
+      iIntros "Hlock". iModIntro. iFrame "Hlock".
+      iIntros "H"; iDestruct ("Hlazy" with "H") as "Hlazy".
+      iLeft. iFrame "Hlazy". clear dependent S. iIntros "AU".
+      iModIntro. iIntros "[Hlocked Hin_lock]".
+      iModIntro. wp_pures; wp_lam; wp_pures.
 
-      wp_bind (Load #(node_next pred +ₗ lvl)). iInv "Hinv" as "Hskip". 
-      iDestruct (has_lvl_inv with "Hskip") as "(Hlvl & Hskip)"; first done.
-      iDestruct "Hlvl" as (S) "(>Hauth & >Hdisj & >Htoks & Hlocks & Hnexts & Hmap)".
-
-      iDestruct (singleton_frag_in with "Hauth Hpred") as %Hpred.
-      rewrite (big_sepS_delete (has_next _ _)) //.
-      iDestruct "Hnexts" as "(Hnext & Hnexts)".
-      iDestruct "Hnext" as (? succ) ">(Hnext & #Hs & #Hsucc & Hkeys)".
-      iDestruct (mapsto_agree with "Hnext Hnext'") as %Hs; inversion Hs; subst.
-
+      wp_bind (Load #(_)). iMod "AU" as (S) "[Hlazy Hclose]".
+      iDestruct (singleton_frag_in with "Hpred Hlazy") as %Hpred.
+      iDestruct (node_has_next with "Hpred Hlazy")
+        as (s succ) "(Hnext & #Hs & #Hsucc & %Hdisj & Hlazy)".
       destruct (decide (k ≤ node_key succ)) as [|Hcase].
-      + clear d; iMod "AU" as (d) "[Hexcl◯ [_ Hclose]]".
-        iDestruct (own_valid_2 with "Hdisj Hkeys") as %[Hdisj _]%ZRange_disj.
-        iDestruct (singleton_frag_in with "Hauth Hsucc") as %Hsucc%elem_of_union.
-        rewrite elem_of_singleton in Hsucc.
+      + iDestruct "Hin_lock" as (?) "[Hnext' Hval]".
+        iDestruct (mapsto_agree with "Hnext Hnext'") as %Hs; 
+          symmetry in Hs; inversion Hs; subst.
 
-        wp_load.
-        iAssert (has_next _ _ pred) with "[Hnext Hkeys]" as "Hnext".
-        { iExists s, succ; iFrame "# ∗". }
-        iCombine "Hnext Hnexts" as "Hnexts".
-        rewrite -big_sepS_delete //.
-
-        iAssert ⌜ lvl = 0 → set_map node_key S = d ⌝%I with "[Hmap Hexcl◯]" as %Heqd.
-        { 
-          iIntros (->); iDestruct "Hmap" as "(Hexcl● & _)".
-          by iDestruct (own_valid_2 with "Hexcl● Hexcl◯") as %<-%excl_auth_agree_L.
-        }
-        iDestruct ("Hclose" with "[Hexcl◯ Hlocked Hnext' Hval]") as ">HΦ"; last iModIntro.
+        wp_load. iDestruct ("Hlazy" with "Hnext") as "Hlazy".
+        iDestruct "Hclose" as "[_ Hclose]".
+        iDestruct ("Hclose" $! pred succ with "[Hlazy]") as ">AP".
         {
-          iFrame "# ∗". iSplit. 
-          + iPureIntro; intros Hneq <-%Heqd Hfalse.
-            by apply (Hdisj k); last (rewrite zrange_spec; lia).
-          + iSplit; first (iPureIntro; lia). iExists γl, l, s; iFrame "# ∗".
+          iDestruct (singleton_frag_in with "Hsucc Hlazy") as %Hsucc.
+          rewrite elem_of_union elem_of_singleton in Hsucc.
+          iFrame "Hlazy"; iPureIntro. intros Hneq Hin%Hdisj. 
+          apply Hin. rewrite zrange_spec; lia.
         }
-
-        iModIntro; iSplitR "HΦ".
-        { iNext; iApply "Hskip"; iExists S; iFrame. }
-        wp_load; wp_let; wp_lam; wp_pures.
+        iMod (atomic_post_commit with "AP") as "HΦ".
+        iModIntro. wp_load; wp_let; wp_lam; wp_pures.
         case_bool_decide; last lia; wp_if.
-        by wp_pure.
-      + wp_load.
-        iAssert (has_next _ _ pred) with "[Hnext Hkeys]" as "Hnext".
-        { iExists s, succ; iFrame "# ∗". }
-        iCombine "Hnext Hnexts" as "Hnexts".
-        rewrite -big_sepS_delete //.
-
-        iModIntro; iSplitR "AU Hlocked Hnext' Hval".
-        { iNext; iApply "Hskip"; iExists S; iFrame. }
-        wp_load; wp_let; wp_lam; wp_pures.
+        wp_pure. iApply "HΦ".
+        iFrame "# ∗". iSplit; first (iPureIntro; lia).
+        iExists s. iFrame "# ∗".
+      + wp_load. iDestruct ("Hlazy" with "Hnext") as "Hlazy".
+        iDestruct "Hclose" as "[Hclose _]"; iDestruct ("Hclose" with "Hlazy") as ">AU".
+        iModIntro. wp_load; wp_let; wp_lam; wp_pures.
         case_bool_decide; first lia; wp_if.
-        wp_apply (release_spec with "[Hlocked Hnext' Hval]").
-        { iFrame "# ∗"; iExists s; iFrame. }
-        iIntros "_"; wp_pures.
+
+        clear dependent S.
+        awp_apply (release_spec with "Hlocked Hin_lock").
+        iApply (aacc_aupd_sub with "[] AU"); try done.
+        { iIntros "!> %S H"; iDestruct (node_has_lock with "Hpred H") as "$". }
+        iIntros (S) "Hlazy". 
+        iDestruct (node_has_lock with "Hpred Hlazy") as "(Hlock & Hlazy)".
+        iAaccIntro with "Hlock".
+        { iIntros "H"; iDestruct ("Hlazy" with "H") as "Hlazy"; iModIntro; iFrame; by iIntros. }
+        iIntros "Hlock". iModIntro. iFrame "Hlock".
+        iIntros "Hlock"; iDestruct ("Hlazy" with "Hlock") as "Hlazy".
+        iLeft. iFrame "Hlazy". clear dependent S. iIntros "AU".
+        iModIntro. iIntros "_".
+        iModIntro. wp_pures.
+
         iDestruct "Hsucc" as "[->|Hsucc]"; first (rewrite /node_key/= in Hcase; lia).
         iApply ("IH" with "[%] [$] AU"); lia.
     Qed.
