jelly_fish/spec/new.v
@@ -1,8 +1,9 @@
-From iris.algebra Require Import gmap gset excl_auth dfrac_agree.
-From iris.base_logic.lib Require Import invariants.
-From iris.heap_lang Require Import proofmode.
+From iris.algebra Require Import auth gset.
+From iris.base_logic.lib Require Import ghost_map.
+From iris.heap_lang Require Import notation.
 
-From SkipList.lib Require Import zrange gmap_extra.
+From SkipList.lib Require Import zrange.
+From SkipList.atomic Require Import weakestpre proofmode lock.
 From SkipList.jelly_fish Require Import code inv.
 
 
@@ -12,47 +13,43 @@ Module NewSpec (Params: SKIP_LIST_PARAMS).
   Export Invariant.
 
   Section proofs.
-    Context `{!heapGS Σ, !skipG Σ} (N: namespace).
+    Context `{!heapGS Σ, !skipG Σ}.
     Local Open Scope Z.
 
-    Theorem initLocks_spec (lvl: Z) (head: node_rep) (t: loc)
-      (Γm: map_gname) (Γ: gmap Z inv_gname) :
+    Theorem alloc_levels (lvl: Z) (head: node_rep) (t: loc)
+      (mΓ: gmap Z lazy_gname) :
       1 ≤ lvl ≤ MAX_HEIGHT + 1 →
       node_key head = INT_MIN →
       t ↦□ rep_to_node tail -∗
-      {{{
-        (node_next head +ₗ lvl) ↦∗ replicate (Z.to_nat (MAX_HEIGHT + 1 - lvl)) #t
+      (node_next head +ₗ lvl) ↦∗ 
+        replicate (Z.to_nat (MAX_HEIGHT + 1 - lvl)) #t -∗
+      (node_lock head +ₗ lvl) ↦∗ 
+        replicate (Z.to_nat (MAX_HEIGHT + 1 - lvl)) #false -∗
+      ([∗ set] i ∈ zrange 0 lvl, is_lazy_list head (mΓ !!! i) (mΓ !!! (i - 1)) i)
+      ==∗
+      ∃ (mΓ': gmap Z lazy_gname),
+        ⌜ mΓ !!! 0 = mΓ' !!! 0 ⌝
         ∗
-        (node_lock head +ₗ lvl) ↦∗ replicate (Z.to_nat (MAX_HEIGHT + 1 - lvl)) #()
-        ∗
-        [∗ set] i ∈ zrange (-1) lvl, lazy_list_inv head Γm Γ i
-      }}}
-        initLocks #(node_lock head) #lvl
-      {{{ Γ, RET #(); skip_list_inv head Γm Γ }}}.
+        [∗ set] i ∈ zrange 0 (MAX_HEIGHT + 1), 
+          is_lazy_list head (mΓ' !!! i) (mΓ' !!! (i - 1)) i.
     Proof.
-      iIntros "%Hlvl %Hmin #Ht %Φ !> (Hnexts & Hlocks & Hskip) HΦ".
-      iRevert (Γ lvl Hlvl) "Hnexts Hlocks Hskip HΦ".
-      iLöb as "IH".
-      iIntros (Γ lvl Hlvl) "Hnexts Hlocks Hskip HΦ".
+      iIntros "%Hlvl %Hmin #Ht".
+      assert (lvl = Z.of_nat (Z.to_nat lvl)) as Heq by lia.
+      remember (Z.to_nat (MAX_HEIGHT + 1 - lvl)) as diff eqn:Hdiff.
+      iRevert (Hlvl); rewrite Heq; clear Heq; iRevert (lvl mΓ Hdiff).
+      iInduction (diff) as [|diff] "Himp"; 
+        iIntros (lvl mΓ) "%Hdiff %Hlvl' Hnexts Hlocks Hskip".
+      + replace (MAX_HEIGHT + 1) with (Z.of_nat (Z.to_nat lvl)) by lia.
+        by iModIntro; iExists mΓ; iFrame.
+      + assert (lvl ≠ MAX_HEIGHT + 1) as Hneq by lia.
 
-      wp_lam. wp_let. wp_pures.
-      case_bool_decide as Hcase; wp_if.
-      + iModIntro; iApply ("HΦ" $! Γ).
-        inversion Hcase; subst; iFrame.
-      + assert (lvl ≠ MAX_HEIGHT + 1) as Hneq by congruence.
-        replace (Z.to_nat (MAX_HEIGHT + 1 - lvl)) with (S (Z.to_nat (MAX_HEIGHT - lvl))) by lia.
-        repeat rewrite replicate_S array_cons.
-        iDestruct "Hlocks" as "(Hlock & Hlocks)".
-        iDestruct "Hnexts" as "((Hnext & Hnext') & Hnexts)".
+        rewrite ?replicate_S ?array_cons ?loc_add_assoc.
+        replace (Z.to_nat lvl + 1) with (Z.of_nat (Z.to_nat (lvl + 1))) by lia.
+        iDestruct "Hnexts" as "[[Hnext Hnext'] Hnexts]".
+        iDestruct "Hlocks" as "[Hlock Hlocks]".
 
-        wp_apply (newlock_spec (in_lock lvl (node_next head)) with "[Hnext']").
-        { iExists t; iFrame; unfold locked_val; by case_decide; first lia. }
-        iIntros (l γl) "#His_lock".
-        wp_store. wp_pures.
-        iMod (mapsto_persist with "Hlock") as "#Hlock".
-
-        iMod (own_alloc (● (∅ : gset node_rep) ⋅ ◯ ∅))
-          as (γauth) "[Hauth _]"; 
+        iMod (own_alloc (● ∅ ⋅ ◯ ∅))
+          as (γauth) "[Hauth _]";
           first by apply auth_both_valid.
         iMod (own_alloc (GSet ∅ ⋅ ZRange (node_key head) (node_key tail)))
           as (γdisj) "[Hdisj Hkeys]";
@@ -60,95 +57,85 @@ Module NewSpec (Params: SKIP_LIST_PARAMS).
         iMod (own_alloc (● GSet ∅ ⋅ ◯ GSet ∅))
           as (γtoks) "[Htoks _]"; 
           first by apply auth_both_valid.
-        set (Γi := mk_inv_gname γauth γdisj γtoks).
-        set (Γ' := <[lvl := Γi]>Γ).
+        set (Γ := mk_lazy_gname γauth γdisj γtoks).
 
-        rewrite ?loc_add_assoc; replace (MAX_HEIGHT - lvl) with (MAX_HEIGHT + 1 - (lvl + 1)) by lia.
-        iApply ("IH" $! Γ' with "[%] Hnexts Hlocks [-HΦ]"); first lia.
-        {
-          rewrite (zrange_split_r _ lvl); last lia.
-          rewrite comm_L big_sepS_insert; last (rewrite zrange_spec; lia).
-          iSplitR "Hskip".
-          + iExists ∅; case_decide; first lia.
-            rewrite right_id_L ?big_sepS_singleton big_sepS_empty set_map_empty lookup_total_insert; iFrame.
-            iSplit; first (iExists γl, l; iFrame "#").
-            iSplit; last done. iExists t, tail; iFrame "# ∗"; by iLeft.
-          + iApply big_sepS_mono; last iFrame.
-            iIntros (m Hm%zrange_spec) "Hlvl".
-            rewrite /lazy_list_inv ?lookup_total_insert_ne //; lia.
-        }
-        iNext; done.
+        iDestruct ("Himp" $! (lvl + 1) (<[lvl := Γ]>mΓ) with "[] [] Hnexts Hlocks [-]")
+          as "Hskip'"; first (iPureIntro; lia); first (iPureIntro; lia);
+          last (rewrite ?lookup_total_insert_ne //; lia).
+
+        replace (Z.of_nat (Z.to_nat (lvl + 1))) with (Z.of_nat (Z.to_nat lvl) + 1) by lia.
+        replace (Z.of_nat (Z.to_nat lvl)) with lvl by lia.
+        rewrite (zrange_split_r _ lvl); last lia.
+        rewrite comm_L big_sepS_insert; last (rewrite zrange_spec; lia).
+        iSplitR "Hskip".
+        - iExists ∅. rewrite /lazy_list ?lookup_total_insert ?set_map_empty 
+            right_id_L ?big_sepS_singleton big_sepS_empty; iFrame "# ∗".
+          iSplitL "Hnext Hkeys"; first (iExists t, tail; iFrame "# ∗"; by iLeft).
+          iSplit; last done. iExists (node_lock head +ₗ lvl), false.
+          rewrite -Qp.quarter_three_quarter; 
+            iDestruct "Hlock" as "[? ?]";
+            rewrite Qp.quarter_three_quarter.
+          iFrame. iSplit; first done. iExists t; iFrame.
+          unfold locked_val; by case_decide; first lia.
+        - iApply big_sepS_mono; last iFrame.
+          iIntros (i Hi%zrange_spec) "Hlazy".
+          rewrite ?lookup_total_insert_ne //; lia.
     Qed.
 
     Theorem new_spec : 
       {{{ True }}}
         new #()
-      {{{ p Γm, RET #p; map_inv N p Γm ∗ map ∅ Γm }}}.
+      {{{ p mΓ, RET #p; vc_map p ∅ mΓ }}}.
     Proof.
       iIntros (Φ) "_ HΦ"; wp_lam; pose proof HMAX_HEIGHT. 
 
       wp_alloc t as "Ht"; iMod (mapsto_persist with "Ht") as "#Ht".
       wp_alloc next as "Hnexts"; first lia. wp_let.
-      wp_alloc locks as "Hlocks"; first lia. wp_let.
+      wp_alloc lock as "Hlocks"; first lia. wp_let.
+      set (head := (INT_MIN, dummy_null, next, lock)).
 
       replace (Z.to_nat (MAX_HEIGHT + 1)) with (S (Z.to_nat MAX_HEIGHT)) by lia.
-      rewrite replicate_S ?array_cons.
-      iDestruct "Hnexts" as "((Hnext & Hnext') & Hnexts)".
-      iDestruct "Hlocks" as "(Hlock & Hlocks)".
+      rewrite ?replicate_S ?array_cons.
+      iDestruct "Hnexts" as "[[Hnext Hnext'] Hnexts]".
+      iDestruct "Hlocks" as "[Hlock Hlocks]".
 
-      wp_lam. wp_let. wp_pures.
-      case_bool_decide as Hcase; first (inversion Hcase; lia).
-      wp_if.
-
-      iMod (own_alloc (●E ∅ ⋅ ◯E ∅))
-        as (γexcl) "[Hexcl● Hexcl◯]";
-        first by apply auth_both_valid.
-      iMod (own_alloc (● DMap ∅ ⋅ ◯ DMap∅))
-        as (γvals) "[Hvals _]"; 
-        first by apply auth_both_valid.
-      set (Γm := mk_map_gname γexcl γvals).
-      set (head := (INT_MIN, dummy_null, next, locks)).
-      wp_apply (newlock_spec (in_lock 0 (node_next head)) with "[Hnext']").
-      { iExists t; rewrite loc_add_0; iFrame. iExists tail; iFrame "#"; by iLeft. }
-      iIntros (l γl) "#His_lock".
-
-      wp_pures; rewrite loc_add_0.
-      wp_store; iMod (mapsto_persist with "Hlock") as "#Hlock".
-      wp_pures; replace (0 + 1) with 1 by lia.
-
+      iMod ghost_map_alloc_empty as (γ) "Hvals".
       iMod (own_alloc (● ∅ ⋅ ◯ ∅))
-        as (γauth) "[Hauth _]"; 
+        as (γauth) "[Hauth _]";
         first by apply auth_both_valid.
       iMod (own_alloc (GSet ∅ ⋅ ZRange (node_key head) (node_key tail)))
         as (γdisj) "[Hdisj Hkeys]";
+          
         first by (pose HMIN_MAX; rewrite ZRange_disj).
       iMod (own_alloc (● GSet ∅ ⋅ ◯ GSet ∅))
         as (γtoks) "[Htoks _]"; 
         first by apply auth_both_valid.
-      set (Γi := mk_inv_gname γauth γdisj γtoks).
-      set (Γ' := ({[ 0 := Γi ]} : gmap Z inv_gname)).
+      set (Γ := mk_lazy_gname γauth γdisj γtoks).
 
-      replace locks with (node_lock head) by auto.
-      replace Γi with (Γ' !!! 0) by set_solver.
-      wp_apply (initLocks_spec _ _ _ Γm Γ' with "Ht [-HΦ Hexcl◯ Hvals]"); first lia; first done.
-      {
-        replace (MAX_HEIGHT + 1 - 1) with MAX_HEIGHT by lia; iFrame. 
-        replace 1 with (0 + 1) by lia; rewrite zrange_split_r; last lia.
-        replace 0 with (-1 + 1) by lia; rewrite zrange_empty_r left_id_L big_sepS_singleton //.
-        iExists ∅; case_decide; last lia.
-        replace (Γ' !!! 0) with Γi by set_solver.
-        rewrite right_id_L ?big_sepS_singleton /own_map big_sepS_empty set_map_empty; iFrame. 
-        iSplit; first (iExists γl, l; rewrite ?loc_add_0; iFrame "#").
-        iExists t, tail; rewrite loc_add_0; iFrame "# ∗"; by iLeft.
-      }
-      iIntros (Γ) "Hskip".
-      iMod (inv_alloc (skipN N) ⊤ (skip_list_inv head Γm Γ) with "Hskip") as "#Hinv".
+      replace MAX_HEIGHT with (MAX_HEIGHT + 1 - 1) by lia.
+      iMod (alloc_levels 1 head t {[ 0 := Γ ]} with "Ht Hnexts Hlocks []") 
+        as (mΓ) "[%HmΓ Hskip]"; first lia; first done;
+        last rewrite lookup_total_singleton in HmΓ.
+      { replace 1 with (0 + 1) by lia; rewrite zrange_empty_r big_sepS_empty //. }
 
       wp_pures; rewrite (fold_rep_to_node head).
       wp_alloc p as "Hp"; iMod (mapsto_persist with "Hp") as "#Hp".
-      iModIntro; iApply ("HΦ" $! _ Γm).
-      iSplit; first by (iExists head, Γ; iFrame "#").
-      rewrite -dom_empty; iFrame.
+      iModIntro; iApply "HΦ".
+      iExists head, ∅. iFrame "Hp Hskip". iSplit; first done.
+      iSplitR "Hvals"; last first.
+      { iExists γ. iFrame "Hvals". rewrite big_sepS_empty. iPureIntro; set_solver. }
+      rewrite -HmΓ /lazy_list ?lookup_total_singleton ?set_map_empty
+        right_id_L ?big_sepS_singleton; iFrame.
+      iSplitR "Hlock Hnext'".
+      { iExists t, tail; rewrite loc_add_0; iFrame "# ∗"; by iLeft. }
+      rewrite -Qp.quarter_three_quarter; 
+        iDestruct "Hlock" as "[? ?]";
+        rewrite Qp.quarter_three_quarter.
+      iSplit; last done. iExists lock, false; iFrame.
+      rewrite loc_add_0; iSplit; first done.
+      iExists t. rewrite loc_add_0; iFrame.
+      unfold locked_val; case_decide; last done.
+      iExists tail. iFrame "Ht". by iLeft.
     Qed.
   End proofs.
 End NewSpec.
